updated most of the revocation to fit the new model, except the lemmas for closing the world again

theories/region_invariants_revocation.v
@@ -1,6 +1,6 @@
 From iris.algebra Require Import gmap agree auth.
 From iris.proofmode Require Import tactics.
-From cap_machine Require Export stdpp_extra iris_extra region_invariants.
+From cap_machine Require Export stdpp_extra iris_extra region_invariants region_invariants_transitions.
 Import uPred.
 
 Section heap.
@@ -19,7 +19,7 @@ Section heap.
   (* --------------------------------------------------------------------------------------------------------- *)
 
   (*
-     Revocation turns every temporary location state to revoked.
+     Revocation turns every temporary/monotemporary location state to revoked.
      Revocation is crucial to privately update state: in general,
      region states are only monotone with regards to public future
      world. To do a private update, we must thus revoke all temp
@@ -32,6 +32,7 @@ Section heap.
   Definition revoke_std_sta : STS_STD → STS_STD :=
     fmap (λ v, match v with
                | Temporary => Revoked
+               | Monotemporary => Revoked
                | _ => v
                end).
   Definition revoke W : WORLD := (revoke_std_sta (std W), loc W).
@@ -43,6 +44,7 @@ Section heap.
     | i :: l' => match fs !! i with
                | Some j => match j with
                           | Temporary => <[i := Revoked]> (revoke_list_std_sta l' fs)
+                          | Monotemporary => <[i := Revoked]> (revoke_list_std_sta l' fs)
                           | _ => (revoke_list_std_sta l' fs)
                           end
                | None => (revoke_list_std_sta l' fs)
@@ -80,7 +82,7 @@ Section heap.
     - apply dom_insert_subseteq.
     - apply not_elem_of_dom in Hdom_sta.
        apply not_elem_of_dom in Hdom_rel.
-       intros j r1 r2 r1' r2' Hr Hr'.
+       intros j r1 r2 r1' r2' r3 r3' Hr Hr'.
        destruct (decide (j = i)).
       + subst. rewrite Hr in Hdom_rel. done.
       + rewrite lookup_insert_ne in Hr'; auto.
@@ -105,7 +107,7 @@ Section heap.
     - rewrite dom_insert_L. set_solver.
     - apply (not_elem_of_dom (D:=gset positive) W.2.1 i) in Hdom_sta.
       apply (not_elem_of_dom (D:=gset positive) W.2.2 i) in Hdom_rel.
-      intros j r1' r2' r1'' r2'' Hr' Hr''.
+      intros j r1' r2' r1'' r2'' r3' r3''  Hr' Hr''.
       destruct (decide (j = i)).
       + subst. rewrite Hdom_rel in Hr'. inversion Hr'.
       + simplify_map_eq. repeat split;auto.
@@ -136,12 +138,36 @@ Section heap.
         left.
   Qed.
 
+  Lemma related_sts_pub_world_revoked_monotemp W a :
+    (std W) !! a = Some Revoked ∨
+    (std W) !! a = Some Monotemporary →
+    related_sts_pub_world W (<s[a:=Monotemporary]s>W).
+  Proof.
+    intros Ha.
+    rewrite /related_sts_pub_world /=.
+    split;[|apply related_sts_pub_refl].
+    rewrite /related_sts_pub. split.
+    - rewrite dom_insert_L. set_solver.
+    - intros i x y Hx Hy.
+      destruct (decide (a = i)).
+      + subst.
+        rewrite Hx in Ha.
+        destruct Ha as [Ha | Ha]; inversion Ha.
+        ++ rewrite lookup_insert in Hy. inversion Hy.
+           right with (Monotemporary);[|left]. constructor.
+        ++ rewrite lookup_insert in Hy. inversion Hy. left.
+      + rewrite lookup_insert_ne in Hy;auto.
+        rewrite Hx in Hy.
+        inversion Hy; subst.
+        left.
+  Qed.
+
   (* The following lemma takes a revoked region and makes it Temporary. *)
 
   Lemma update_region_revoked_temp_pwl E W l p v φ `{∀ Wv, Persistent (φ Wv)} :
     (std W) !! l = Some Revoked →
     p ≠ O → pwl p = true →
-    future_pub_mono φ v -∗
+    future_pub_plus_mono φ v -∗
     sts_full_world W -∗
     region W -∗
     l ↦ₐ[p] v -∗ φ (W,v) -∗ rel l p φ ={E}=∗ region (<s[l := Temporary ]s>W)
@@ -162,11 +188,13 @@ Section heap.
     iMod (sts_update_std _ _ _ Temporary with "Hsts Hstate") as "[Hsts Hstate]".
     assert (related_sts_pub_world W (<s[l := Temporary ]s> W)) as Hrelated.
     { apply related_sts_pub_world_revoked_temp; auto. }
+    assert (related_sts_pub_plus_world W (<s[l := Temporary ]s> W)) as Hrelated'.
+    { apply related_sts_pub_pub_plus_world;auto. }
     iDestruct (region_map_monotone _ _ _ _ Hrelated with "Hr") as "Hr".
-    iDestruct ("Hmono" $! _ _ Hrelated with "Hφ") as "Hφ'".
+    iDestruct ("Hmono" $! _ _ Hrelated' with "Hφ") as "Hφ'".
     assert (is_Some (M !! l)) as [x Hsome].
     { apply elem_of_gmap_dom. rewrite -Hdom. apply elem_of_gmap_dom. eauto. }
-    iDestruct (region_map_delete_nonstatic with "Hr") as "Hr"; [intros m;intros Hcontr;congruence|].
+    iDestruct (region_map_delete_nonstatic with "Hr") as "Hr";[intros m;split;intros Hcontr;congruence|].
     iDestruct (region_map_insert_nonstatic Temporary with "Hr") as "Hr";auto.
     iDestruct (big_sepM_delete _ _ l _ Hsome with "[Hl Hstate $Hr]") as "Hr".
     { iExists Temporary. iFrame. iSplitR;[iPureIntro;apply lookup_insert|].
@@ -208,7 +236,7 @@ Section heap.
     assert (related_sts_priv_world W (<s[l := Temporary ]s> W)) as Hrelated'.
     { apply related_sts_pub_priv_world. auto. }
     iDestruct (region_map_monotone _ _ _ _ Hrelated with "Hr") as "Hr".
-    iDestruct (region_map_delete_nonstatic with "Hr") as "Hr"; [intros m;intros Hcontr;congruence|].
+    iDestruct (region_map_delete_nonstatic with "Hr") as "Hr"; [intros m;split;intros Hcontr;congruence|].
     iDestruct (region_map_insert_nonstatic Temporary with "Hr") as "Hr";auto.
     iDestruct ("Hmono" $! _ _ Hrelated' with "Hφ") as "Hφ'".
     assert (is_Some (M !! l)) as [x Hsome].
@@ -220,7 +248,102 @@ Section heap.
       destruct (pwl p); iFrame "#".
       iIntros (W' W'' Hrelated''). iModIntro. iIntros "HφW'".
       iApply ("Hmono" with "[] HφW'").
-      iPureIntro. apply related_sts_pub_priv_world; auto.
+      iPureIntro. apply related_sts_pub_plus_priv_world; auto.
+    }
+    rewrite /std_update /=. iFrame "Hsts".
+    iExists M. iFrame. rewrite -HMeq. iFrame.
+    iModIntro. iExists _. iFrame. iPureIntro.
+    apply insert_id in Hsome. apply insert_id in Hl. rewrite -Hsome -Hl. split.
+    - repeat rewrite dom_insert_L;rewrite Hdom;set_solver.
+    - repeat rewrite dom_insert_L;rewrite Hdom';set_solver.
+  Qed.
+
+  Lemma update_region_revoked_monotemp_pwl E W l p v φ `{∀ Wv, Persistent (φ Wv)} :
+    (std W) !! l = Some Revoked →
+    p ≠ O → pwl p = true →
+    future_pub_a_mono l φ v -∗
+    sts_full_world W -∗
+    region W -∗
+    l ↦ₐ[p] v -∗ φ (W,v) -∗ rel l p φ ={E}=∗ region (<s[l := Monotemporary ]s>W)
+                             ∗ sts_full_world (<s[l := Monotemporary ]s>W).
+  Proof.
+    iIntros (Hrev HO Hpwl) "#Hmono Hsts Hreg Hl #Hφ #Hrel".
+    rewrite region_eq /region_def.
+    iDestruct "Hreg" as (M Mρ) "(Hγrel & #Hdom & #Hdom' & Hpreds)".
+    iDestruct "Hdom" as %Hdom. iDestruct "Hdom'" as %Hdom'.
+    rewrite RELS_eq /RELS_def.
+    rewrite rel_eq /rel_def REL_eq /REL_def. iDestruct "Hrel" as (γ) "[HREL Hsaved]".
+    iDestruct (reg_in γrel (M) with "[$Hγrel $HREL]") as %HMeq.
+    rewrite /region_map_def HMeq big_sepM_insert; [|by rewrite lookup_delete].
+    iDestruct "Hpreds" as "[Hl' Hr]".
+    iDestruct "Hl'" as (ρ Hl) "[Hstate Hresources]".
+    iDestruct (sts_full_state_std with "Hsts Hstate") as %Hρ.
+    rewrite Hrev in Hρ. inversion Hρ as [Hρrev]. subst.
+    iMod (sts_update_std _ _ _ Monotemporary with "Hsts Hstate") as "[Hsts Hstate]".
+    assert (related_sts_pub_world W (<s[l := Monotemporary ]s> W)) as Hrelated.
+    { apply related_sts_pub_world_revoked_monotemp; auto. }
+    assert (related_sts_a_world W (<s[l := Monotemporary ]s> W) l) as Hrelated'.
+    { apply related_sts_pub_a_world; auto. }
+    iDestruct (region_map_monotone _ _ _ _ Hrelated with "Hr") as "Hr".
+    iDestruct ("Hmono" $! _ _ Hrelated' with "Hφ") as "Hφ'".
+    assert (is_Some (M !! l)) as [x Hsome].
+    { apply elem_of_gmap_dom. rewrite -Hdom. apply elem_of_gmap_dom. eauto. }
+    iDestruct (region_map_delete_nonstatic with "Hr") as "Hr"; [intros m;split;intros Hcontr;congruence|].
+    iDestruct (region_map_insert_nonstatic Monotemporary with "Hr") as "Hr";auto.
+    iDestruct (big_sepM_delete _ _ l _ Hsome with "[Hl Hstate $Hr]") as "Hr".
+    { iExists Monotemporary. iFrame. iSplitR;[iPureIntro;apply lookup_insert|].
+      iExists γ, p, φ. rewrite HMeq lookup_insert in Hsome.
+      inversion Hsome. repeat (iSplit; auto). iExists _. iFrame.
+      iSplit;auto. rewrite Hpwl. iFrame "#". }
+    rewrite /std_update /=. iFrame "Hsts".
+    iExists M. iFrame. rewrite -HMeq. iFrame.
+    iModIntro. iExists _. iFrame. iPureIntro.
+    apply insert_id in Hsome. apply insert_id in Hl. rewrite -Hsome -Hl. split.
+    - repeat rewrite dom_insert_L;rewrite Hdom;set_solver.
+    - repeat rewrite dom_insert_L;rewrite Hdom';set_solver.
+  Qed.
+
+   Lemma update_region_revoked_monotemp_nwl E W l p v φ `{∀ Wv, Persistent (φ Wv)} :
+    (std W) !! l = Some Revoked →
+    p ≠ O →
+    future_priv_mono φ v -∗
+    sts_full_world W -∗
+    region W -∗
+    l ↦ₐ[p] v -∗ φ (W,v) -∗ rel l p φ ={E}=∗ region (<s[l := Monotemporary ]s>W)
+                             ∗ sts_full_world (<s[l := Monotemporary ]s>W).
+  Proof.
+    iIntros (Hrev HO) "#Hmono Hsts Hreg Hl #Hφ #Hrel".
+    rewrite region_eq /region_def.
+    iDestruct "Hreg" as (M Mρ) "(Hγrel & #Hdom & #Hdom' & Hpreds)".
+    iDestruct "Hdom" as %Hdom. iDestruct "Hdom'" as %Hdom'.
+    rewrite RELS_eq /RELS_def.
+    rewrite rel_eq /rel_def REL_eq /REL_def. iDestruct "Hrel" as (γ) "[HREL Hsaved]".
+    iDestruct (reg_in γrel (M) with "[$Hγrel $HREL]") as %HMeq.
+    rewrite /region_map_def HMeq big_sepM_insert; [|by rewrite lookup_delete].
+    iDestruct "Hpreds" as "[Hl' Hr]".
+    iDestruct "Hl'" as (ρ Hl) "[Hstate Hresources]".
+    iDestruct (sts_full_state_std with "Hsts Hstate") as %Hρ.
+    rewrite Hrev in Hρ. inversion Hρ as [Hρrev]. subst.
+    iMod (sts_update_std _ _ _ Monotemporary with "Hsts Hstate") as "[Hsts Hstate]".
+    assert (related_sts_pub_world W (<s[l := Monotemporary ]s> W)) as Hrelated.
+    { apply related_sts_pub_world_revoked_monotemp; auto. }
+    assert (related_sts_priv_world W (<s[l := Monotemporary ]s> W)) as Hrelated'.
+    { apply related_sts_pub_priv_world. auto. }
+    iDestruct (region_map_monotone _ _ _ _ Hrelated with "Hr") as "Hr".
+    iDestruct (region_map_delete_nonstatic with "Hr") as "Hr"; [intros m;split;intros Hcontr;congruence|].
+    iDestruct (region_map_insert_nonstatic Monotemporary with "Hr") as "Hr";auto.
+    iDestruct ("Hmono" $! _ _ Hrelated' with "Hφ") as "Hφ'".
+    assert (is_Some (M !! l)) as [x Hsome].
+    { apply elem_of_gmap_dom. rewrite -Hdom. apply elem_of_gmap_dom. eauto. }
+    iDestruct (big_sepM_delete _ _ l _ Hsome with "[Hl Hstate $Hr]") as "Hr".
+    { iExists Monotemporary. iFrame. iSplitR;[iPureIntro;apply lookup_insert|].
+      iExists γ, p, φ. rewrite HMeq lookup_insert in Hsome.
+      inversion Hsome. repeat (iSplit; auto). iExists _. iFrame. iSplit;auto.
+      destruct (pwl p); iFrame "#".
+      iIntros (W' W'' Hrelated''). iModIntro. iIntros "HφW'".
+      iApply ("Hmono" with "[] HφW'").
+      iPureIntro. apply related_sts_pub_plus_priv_world.
+      eapply related_sts_a_pub_plus_world;eauto.
     }
     rewrite /std_update /=. iFrame "Hsts".
     iExists M. iFrame. rewrite -HMeq. iFrame.
@@ -236,6 +359,7 @@ Section heap.
   Definition revoke_i i :=
     match i with
     | Temporary => Revoked
+    | Monotemporary => Revoked
     | _ => i
     end.
 
@@ -252,7 +376,7 @@ Section heap.
       { destruct (in_dec addr_eq_dec i (a :: l)).
         + destruct i0 as [A | A].
           * subst i. simpl. rewrite H3.
-            destruct j;[rewrite lookup_insert;auto|rewrite IHl H3; destruct (in_dec addr_eq_dec a l);auto..].
+            destruct j;[rewrite lookup_insert;auto|rewrite lookup_insert;auto|rewrite IHl H3; destruct (in_dec addr_eq_dec a l);auto..].
           * simpl.
             case_eq (Wstd_sta !! a); intros.
             { destruct (decide (Temporary = r)).
@@ -260,7 +384,12 @@ Section heap.
                 { subst;rewrite lookup_insert. by simplify_map_eq. }
                 { rewrite lookup_insert_ne;auto. rewrite IHl H3.
                   destruct (in_dec addr_eq_dec i l);[auto|contradiction]. }
-              - destruct r; try contradiction; rewrite IHl H3;
+              - destruct (decide (Monotemporary = r)). 
+                { subst. destruct (decide (i = a)).
+                  - subst. rewrite lookup_insert. by simplify_map_eq.
+                  - rewrite lookup_insert_ne//. rewrite IHl H3.
+                    destruct (in_dec addr_eq_dec i l);[auto|contradiction]. }
+                destruct r; try contradiction; rewrite IHl H3;
                 destruct (in_dec addr_eq_dec i l); tauto. }
             { rewrite IHl H3.
               destruct (in_dec addr_eq_dec i l); tauto. }
@@ -271,7 +400,11 @@ Section heap.
                 destruct (in_dec addr_eq_dec i l); auto.
                 elim n. right; auto.
               - red; intro. elim n; left; auto. }
-            { destruct r; try contradiction; rewrite IHl H3;
+            { destruct (decide (Monotemporary = r)). 
+              { subst. rewrite lookup_insert_ne.
+                rewrite IHl H3. destruct (in_dec addr_eq_dec i l); auto.
+                elim n. right; auto. red; intro. elim n; left; auto. }
+              destruct r; try contradiction; rewrite IHl H3;
               destruct (in_dec addr_eq_dec i l); auto;
               elim n; right; auto. }
           * rewrite IHl H3.
@@ -282,7 +415,10 @@ Section heap.
           destruct (decide (Temporary = r)); intros.
           + subst. rewrite lookup_insert_ne; auto.
             rewrite IHl H3; auto.
-          + destruct r; try contradiction; rewrite IHl H3; auto.
+          + destruct (decide (Monotemporary = r)); intros.
+            subst. rewrite lookup_insert_ne;auto.
+            rewrite IHl H3;auto.
+            destruct r; try contradiction; rewrite IHl H3; auto.
         - rewrite IHl H3; auto. }
   Qed.
 
@@ -310,8 +446,15 @@ Section heap.
       elim n. eapply elem_of_list_In.
       eapply elem_of_list_fmap. exists (i, Temporary).
       split; auto.
-    - destruct (in_dec addr_eq_dec i (map_to_list Wstd_sta).*1); auto.
-      destruct x;auto. contradiction.
+    - destruct (decide (Monotemporary = x)).
+      + subst x. eapply elem_of_map_to_list in Hwstd as Hx.
+        destruct (in_dec addr_eq_dec i (map_to_list Wstd_sta).*1); auto.
+        apply leibniz_equiv_iff. 
+        elim n0. eapply elem_of_list_In.
+        eapply elem_of_list_fmap. exists (i, Monotemporary).
+        split; auto.
+      + destruct (in_dec addr_eq_dec i (map_to_list Wstd_sta).*1); auto.
+        destruct x;auto; try contradiction.
     - apply leibniz_equiv_iff. auto.
       Unshelve. apply _.
   Qed.
@@ -375,6 +518,18 @@ Section heap.
       eapply map_to_list_fst. eexists; by apply elem_of_map_to_list.
   Qed.
 
+  Lemma revoke_lookup_Monotemp Wstd_sta i :
+    (Wstd_sta !! i = Some Monotemporary) →
+    (revoke_std_sta Wstd_sta) !! i = Some Revoked.
+  Proof.
+    rewrite revoke_list_dom_std_sta. intros Hsome.
+    rewrite revoke_list_std_sta_spec Hsome.
+    destruct (in_dec addr_eq_dec i (map_to_list Wstd_sta).*1) eqn:HH.
+    - rewrite /revoke_i HH. auto.
+    - elim n. eapply elem_of_list_In.
+      eapply map_to_list_fst. eexists; by apply elem_of_map_to_list.
+  Qed.
+
   Lemma revoke_lookup_Revoked Wstd_sta i :
     (Wstd_sta !! i = Some Revoked) →
     (revoke_std_sta Wstd_sta) !! i = Some Revoked.
@@ -411,9 +566,33 @@ Section heap.
       eapply map_to_list_fst. eexists; by apply elem_of_map_to_list.
   Qed.
 
+  Lemma revoke_lookup_Monostatic Wstd_sta i m :
+    (Wstd_sta !! i = Some (Monostatic m)) →
+    (revoke_std_sta Wstd_sta) !! i = Some (Monostatic m).
+  Proof.
+    rewrite revoke_list_dom_std_sta. intros Hsome.
+    rewrite revoke_list_std_sta_spec Hsome.
+    destruct (in_dec addr_eq_dec i (map_to_list Wstd_sta).*1) eqn:HH.
+    - rewrite /revoke_i HH. auto.
+    - elim n. eapply elem_of_list_In.
+      eapply map_to_list_fst. eexists; by apply elem_of_map_to_list.
+  Qed.
+
+  Lemma revoke_lookup_Uninitialized Wstd_sta i w :
+    (Wstd_sta !! i = Some (Uninitialized w)) →
+    (revoke_std_sta Wstd_sta) !! i = Some (Uninitialized w).
+  Proof.
+    rewrite revoke_list_dom_std_sta. intros Hsome.
+    rewrite revoke_list_std_sta_spec Hsome.
+    destruct (in_dec addr_eq_dec i (map_to_list Wstd_sta).*1) eqn:HH.
+    - rewrite /revoke_i HH. auto.
+    - elim n. eapply elem_of_list_In.
+      eapply map_to_list_fst. eexists; by apply elem_of_map_to_list.
+  Qed.
+
   Lemma revoke_list_lookup_non_temp (Wstd_sta : STS_STD) (l : list Addr) (i : Addr) (ρ : region_type) :
     i ∈ l →
-    (revoke_list_std_sta l Wstd_sta) !! i = Some ρ → ρ ≠ Temporary.
+    (revoke_list_std_sta l Wstd_sta) !! i = Some ρ → ρ ≠ Temporary ∧ ρ ≠ Monotemporary.
   Proof.
     intros Hin Hsome.
     rewrite revoke_list_std_sta_spec in Hsome.
@@ -423,11 +602,13 @@ Section heap.
     inv Hsome. rewrite /revoke_i.
     destruct (decide (Temporary = r)).
     - destruct r;auto;contradiction.
-    - destruct r;[contradiction|auto..].
+    - destruct (decide (Monotemporary = r)).
+      + destruct r;auto;contradiction.
+      + destruct r;[contradiction|auto..].
   Qed.
 
   Lemma revoke_std_sta_lookup_non_temp Wstd_sta (i : Addr) (ρ : region_type) :
-    (revoke_std_sta Wstd_sta) !! i = Some ρ → ρ ≠ Temporary.
+    (revoke_std_sta Wstd_sta) !! i = Some ρ → ρ ≠ Temporary ∧ ρ ≠ Monotemporary.
   Proof.
     intros Hin.
     rewrite revoke_list_dom_std_sta in Hin.
@@ -441,7 +622,7 @@ Section heap.
   Qed.
 
   Lemma revoke_lookup_non_temp W (i : Addr) (ρ : region_type) :
-    (std (revoke W)) !! i = Some ρ → ρ ≠ Temporary.
+    (std (revoke W)) !! i = Some ρ → ρ ≠ Temporary ∧ ρ ≠ Monotemporary.
   Proof.
     intros Hin.
     rewrite revoke_list_dom in Hin.
@@ -497,9 +678,10 @@ Section heap.
 
   Lemma revoke_monotone_lookup_same (Wstd_sta : gmap Addr region_type) i :
     Wstd_sta !! i ≠ Some Temporary ->
+    Wstd_sta !! i ≠ Some Monotemporary →
     revoke_std_sta Wstd_sta !! i = Wstd_sta !! i.
   Proof.
-    intros Hneq.
+    intros Hneq Hneq'.
     induction Wstd_sta using map_ind.
     - rewrite /revoke_std_sta lookup_empty lookup_fmap. eauto.
     - destruct (decide (i0 = i)).
@@ -507,30 +689,25 @@ Section heap.
         rewrite /revoke_std_sta fmap_insert lookup_insert lookup_insert /=.
         f_equiv.
         destruct x eqn:Hcontr; auto.
-        contradiction.
-      + rewrite lookup_insert_ne in Hneq;auto.
+        contradiction. simplify_map_eq. 
+      + simplify_map_eq. 
         rewrite /revoke_std_sta fmap_insert lookup_insert_ne;auto.
-        rewrite lookup_insert_ne;auto.
   Qed.
 
   Lemma revoke_monotone_lookup_same' (W:WORLD) (i: Addr) :
     std W !! i ≠ Some Temporary ->
+    std W !! i ≠ Some Monotemporary ->
     std (revoke W) !! i = std W !! i.
   Proof. cbn. eauto using revoke_monotone_lookup_same. Qed.
 
   Lemma anti_revoke_lookup_Revoked Wstd_sta i :
     (revoke_std_sta Wstd_sta) !! i = Some Revoked ->
-    (Wstd_sta !! i = Some Revoked) ∨ (Wstd_sta !! i = Some Temporary).
+    (Wstd_sta !! i = Some Revoked) ∨ (Wstd_sta !! i = Some Temporary) ∨ (Wstd_sta !! i = Some Monotemporary).
   Proof.
     intros Hrev.
     assert (is_Some (Wstd_sta !! i)) as [x Hx];[apply revoke_std_sta_lookup_Some;eauto|].
-    destruct x;subst;auto.
-    - assert (Wstd_sta !! i ≠ Some Temporary) as Hntemp.
-      { intros Hcontr; subst. rewrite Hx in Hcontr. inversion Hcontr. }
-      apply revoke_monotone_lookup_same in Hntemp. rewrite Hrev in Hntemp. auto.
-    - assert (Wstd_sta !! i ≠ Some Temporary) as Hntemp.
-      { intros Hcontr; subst. rewrite Hx in Hcontr. inversion Hcontr. }
-      apply revoke_monotone_lookup_same in Hntemp. rewrite Hrev in Hntemp. auto.
+    destruct x;subst;auto;
+      rewrite revoke_monotone_lookup_same in Hrev;auto;rewrite Hx;auto.
   Qed.
 
   Lemma revoke_dom_eq Wstd_sta :
@@ -570,7 +747,7 @@ Section heap.
     Wstd_sta !! i = Some x -> Wstd_sta' !! i = Some y ->
     (revoke_std_sta Wstd_sta) !! i = Some x' → (revoke_std_sta Wstd_sta') !! i = Some y' →
     rtc (std_rel_priv) x y →
-    rtc (λ x0 y0 : region_type, std_rel_pub x0 y0 ∨ std_rel_priv x0 y0) x' y'.
+    rtc (λ x0 y0 : region_type, std_rel_pub x0 y0 ∨ std_rel_pub_plus x0 y0 ∨ std_rel_priv x0 y0) x' y'.
   Proof.
     intros Hx Hy Hx' Hy' Hrtc.
     induction Hrtc as [Hrefl | j k h Hjk].
@@ -583,24 +760,33 @@ Section heap.
         apply revoke_lookup_Perm in Hy as Hyperm.
         rewrite Hxtemp in Hx'. rewrite Hyperm in Hy'.
         inversion Hx'; inversion Hy'; simplify_eq.
-        right with Permanent; [|left]. right. constructor.
+        right with Permanent; [|left]. left. constructor.
       + subst.
         apply revoke_lookup_Temp in Hx as Hxtemp.
         rewrite Hxtemp in Hx'. inversion Hx'; simplify_eq.
         destruct h.
         * apply revoke_lookup_Temp in Hy as Hytemp.
+          rewrite Hytemp in Hy'. inversion Hy'; simplify_eq.
+          left.
+        * apply revoke_lookup_Monotemp in Hy as Hytemp.
           rewrite Hytemp in Hy'. inversion Hy'; simplify_eq.
           left.
         * apply revoke_lookup_Perm in Hy as Hytemp.
           rewrite Hytemp in Hy'. inversion Hy'; simplify_eq.
           right with Permanent; [|left].
-          right. constructor.
+          left. constructor.
         * apply revoke_lookup_Revoked in Hy as Hytemp.
           rewrite Hytemp in Hy'. inversion Hy'; simplify_eq.
           left.
         * apply revoke_lookup_Static in Hy as Hytemp.
           rewrite Hytemp in Hy'. inversion Hy'; simplify_eq.
-          apply rtc_or_intro_l. auto.
+          apply rtc_or_intro_l. apply rtc_or_intro_l. auto.
+        * apply revoke_lookup_Monostatic in Hy as Hytemp.
+          rewrite Hytemp in Hy'. inversion Hy'; simplify_eq.
+          apply rtc_or_intro_l. apply rtc_or_intro_l. auto.
+        * apply revoke_lookup_Uninitialized in Hy as Hytemp.
+          rewrite Hytemp in Hy'. inversion Hy'; simplify_eq.
+          apply rtc_or_intro_l. apply rtc_or_intro_l. auto.
       + subst.
         apply revoke_lookup_Temp in Hx as Hxtemp.
         rewrite Hxtemp in Hx'. inversion Hx'; simplify_eq.
@@ -608,9 +794,12 @@ Section heap.
         * apply revoke_lookup_Temp in Hy as Hytemp.
           rewrite Hytemp in Hy'. inversion Hy'; simplify_eq.
           left.
+        * apply revoke_lookup_Monotemp in Hy as Hytemp.
+          rewrite Hytemp in Hy'. inversion Hy'; simplify_eq.
+          left.
         * apply revoke_lookup_Perm in Hy as Hytemp.
           rewrite Hytemp in Hy'. inversion Hy'; simplify_eq.
-          right with Permanent; [|left]. right. constructor.
+          right with Permanent; [|left]. left. constructor.
         * apply revoke_lookup_Revoked in Hy as Hytemp.
           rewrite Hytemp in Hy'. inversion Hy'; simplify_eq.
           left.
@@ -619,21 +808,51 @@ Section heap.
           right with Temporary.
           { left. constructor. }
           right with (Static g0);[|by left].
-          right. constructor.
-      + apply std_rel_priv_rtc_Permanent in Hrtc; auto; subst.
-        apply revoke_lookup_Revoked in Hx as Hxtemp.
-        apply revoke_lookup_Perm in Hy as Hyperm.
-        rewrite Hxtemp in Hx'. rewrite Hyperm in Hy'.
-        inversion Hx'; inversion Hy'; simplify_eq.
-        right with Permanent; [|left].
-        right. constructor.
+          right. right. constructor.
+        * apply revoke_lookup_Monostatic in Hy as Hytemp.
+          rewrite Hytemp in Hy'. inversion Hy'; simplify_eq.
+          right with Monotemporary.
+          { left. constructor. }
+          right with (Monostatic g0);[|by left].
+          right. right. constructor.
+        * apply revoke_lookup_Uninitialized in Hy as Hytemp.
+          rewrite Hytemp in Hy'. inversion Hy'; simplify_eq.
+          right with Monotemporary.
+          { left. constructor. }
+          right with (Uninitialized w);[|by left].
+          right. left. constructor.
+      + apply std_rel_priv_rtc_Temporary in Hrtc as [-> | [-> | [-> | [? ->] ] ] ]; auto; subst.
+        * apply revoke_lookup_Monotemp in Hx as Hxtemp.
+          apply revoke_lookup_Temp in Hy as Hytemp.
+          simplify_eq. left.
+        * apply revoke_lookup_Monotemp in Hx as Hxtemp.
+          apply revoke_lookup_Perm in Hy as Hytemp.
+          simplify_eq. right with Permanent.
+          left. constructor. left.
+        * apply revoke_lookup_Monotemp in Hx as Hxtemp.
+          apply revoke_lookup_Revoked in Hy as Hytemp.
+          simplify_eq. left.
+        * apply revoke_lookup_Monotemp in Hx as Hxtemp.
+          apply revoke_lookup_Static in Hy as Hytemp.
+          simplify_eq. right with Temporary.
+          left;constructor. eright;[|left]. right;right;constructor.
+      + apply std_rel_priv_rtc_Revoked in Hrtc;auto;subst.
+        apply revoke_lookup_Monotemp in Hx as Hxtemp.
+        apply revoke_lookup_Revoked in Hy as Hyperm.
+        simplify_eq. left.
+      + subst. eapply std_rel_priv_rtc_Monostatic in Hrtc;auto;subst.
+        apply revoke_lookup_Monotemp in Hx as Hxtemp.
+        apply revoke_lookup_Monostatic in Hy as Hyperm.
+        simplify_eq. right with Monotemporary.
+        left. constructor. eright;[|left].
+        right. right. constructor.
   Qed.
 
   Lemma std_rel_pub_monotone x y x' y' Wstd_sta Wstd_sta' i :
     Wstd_sta !! i = Some x -> Wstd_sta' !! i = Some y ->
     (revoke_std_sta Wstd_sta) !! i = Some x' → (revoke_std_sta Wstd_sta') !! i = Some y' →
     rtc std_rel_pub x y →
-    rtc (λ x0 y0 : region_type, std_rel_pub x0 y0 ∨ std_rel_priv x0 y0) x' y'.
+    rtc (λ x0 y0 : region_type, std_rel_pub x0 y0 ∨ std_rel_pub_plus x0 y0 ∨ std_rel_priv x0 y0) x' y'.
   Proof.
     intros Hx Hy Hx' Hy' Hrtc.
     induction Hrtc as [Hrefl | j k h Hjk].
@@ -647,15 +866,29 @@ Section heap.
         rewrite Hxtemp in Hx'. rewrite Hyperm in Hy'.
         inversion Hx'; inversion Hy'; simplify_eq.
         left.
+      + apply std_rel_pub_rtc_Monotemporary in Hrtc; auto. subst.
+        apply revoke_lookup_Revoked in Hx as Hxtemp.
+        apply revoke_lookup_Monotemp in Hy as Hyperm.
+        simplify_eq. left.
+      + apply std_rel_pub_rtc_Permanent in Hrtc; auto. subst.
+        apply revoke_lookup_Revoked in Hx as Hxtemp.
+        apply revoke_lookup_Perm in Hy as Hyperm.
+        simplify_eq. eright;[|left]. left. constructor.
       + apply std_rel_pub_rtc_Temporary in Hrtc; auto. subst.
         apply revoke_lookup_Static in Hx as Hxtemp.
         apply revoke_lookup_Temp in Hy as Hyperm.
-        rewrite Hxtemp in Hx'. rewrite Hyperm in Hy'.
-        inversion Hx'; inversion Hy'; simplify_eq.
-        right with Temporary.
-        { left. constructor. }
-        right with Revoked;[|left].
-        right. constructor.
+        simplify_eq. right with Temporary. left;constructor.
+        eright;[|left]. right. right. constructor.
+      + subst. apply std_rel_pub_rtc_Monotemporary in Hrtc; auto. subst.
+        apply revoke_lookup_Monostatic in Hx as Hxtemp.
+        apply revoke_lookup_Monotemp in Hy as Hyperm.
+        simplify_eq. right with Monotemporary. left;constructor.
+        eright;[|left]. right. right. constructor.
+      + subst. apply std_rel_pub_rtc_Monotemporary in Hrtc; auto. subst.
+        apply revoke_lookup_Uninitialized in Hx as Hxtemp.
+        apply revoke_lookup_Monotemp in Hy as Hyperm.
+        simplify_eq. right with Monotemporary. left;constructor.
+        eright;[|left]. right. right. constructor.
   Qed.
 
   Ltac revoke_i W1 W2 i :=
@@ -664,39 +897,87 @@ Section heap.
            , H' : W2 !! i = Some _ |- _ =>
        let Hxtemp := fresh "Hxtemp" in
        let Hytemp := fresh "Hytemp" in
-      try (apply revoke_lookup_Temp in H as Hxtemp);
-      try (apply revoke_lookup_Perm in H as Hxtemp);
-      try (apply revoke_lookup_Revoked in H as Hxtemp);
-      try (eapply revoke_lookup_Static in H as Hxtemp);
-      try (apply revoke_lookup_Temp in H' as Hytemp);
-      try (apply revoke_lookup_Perm in H' as Hytemp);
-      try (eapply revoke_lookup_Static in H' as Hytemp);
-      try (apply revoke_lookup_Revoked in H' as Hytemp);simplify_eq
-    end).
+       try (apply revoke_lookup_Temp in H as Hxtemp);
+       try (apply revoke_lookup_Monotemp in H as Hxtemp);
+       try (apply revoke_lookup_Perm in H as Hxtemp);
+       try (apply revoke_lookup_Revoked in H as Hxtemp);
+       try (eapply revoke_lookup_Static in H as Hxtemp);
+       try (eapply revoke_lookup_Uninitialized in H as Hxtemp);
+       try (eapply revoke_lookup_Monostatic in H as Hxtemp);
+       try (apply revoke_lookup_Temp in H' as Hytemp);
+       try (apply revoke_lookup_Monotemp in H' as Hytemp);
+       try (apply revoke_lookup_Perm in H' as Hytemp);
+       try (eapply revoke_lookup_Static in H' as Hytemp);
+       try (eapply revoke_lookup_Uninitialized in H' as Hytemp);
+       try (eapply revoke_lookup_Monostatic in H' as Hytemp);
+       try (apply revoke_lookup_Revoked in H' as Hytemp);simplify_eq
+     end).
 
   Lemma std_rel_monotone x y x' y' Wstd_sta Wstd_sta' i :
     Wstd_sta !! i = Some x -> Wstd_sta' !! i = Some y ->
     (revoke_std_sta Wstd_sta) !! i = Some x' → (revoke_std_sta Wstd_sta') !! i = Some y' →
-    rtc (λ x0 y0 : region_type, std_rel_pub x0 y0 ∨ std_rel_priv x0 y0) x y →
-    rtc (λ x0 y0 : region_type, std_rel_pub x0 y0 ∨ std_rel_priv x0 y0) x' y'.
+    rtc (λ x0 y0 : region_type, std_rel_pub x0 y0 ∨ std_rel_pub_plus x0 y0 ∨ std_rel_priv x0 y0) x y →
+    rtc (λ x0 y0 : region_type, std_rel_pub x0 y0 ∨ std_rel_pub_plus x0 y0 ∨ std_rel_priv x0 y0) x' y'.
   Proof.
     intros Hx Hy Hx' Hy' Hrtc.
     induction Hrtc as [Hrefl | j k h Hjk].
     - simplify_eq. rewrite -Hx in Hy.
       apply revoke_monotone_lookup in Hy.
       rewrite Hx' Hy' in Hy. inversion Hy. left.
-    - destruct Hjk as [Hjk | Hjk].
+    - destruct Hjk as [Hjk | [Hjk | Hjk] ].
       + destruct j,k; inversion Hjk; try discriminate; auto.
-        * destruct h;revoke_i Wstd_sta Wstd_sta' i;
-            [|right with Temporary;[left;constructor|eright;[right;constructor|left] ]..].
-          eapply std_rel_pub_monotone;[apply Hx|apply Hy|..]; auto.
-          right with Temporary;[|left]. constructor.
-        * subst.
-          destruct h; revoke_i Wstd_sta Wstd_sta' i; try left;
-            [right with Temporary;[left;constructor|eright;[right;constructor|left] ]..].
+        * destruct h;revoke_i Wstd_sta Wstd_sta' i;try left.
+          eright;[left;constructor|left].
+          right with Temporary. left;constructor.
+          eright;[right;right;constructor|left].
+          right with Temporary. left;constructor.
+          right with Revoked. right;right;constructor.
+          right with Monotemporary. left;constructor.
+          eright;[right;right;constructor|left].
+          right with Monotemporary. left;constructor.
+          eright;[right;left;constructor|left].
+        * destruct h;revoke_i Wstd_sta Wstd_sta' i;try left.
+          eright;[left;constructor|left].
+          right with Temporary. left;constructor.
+          eright;[right;right;constructor|left].
+          right with Monotemporary. left;constructor.
+          eright;[right;right;constructor|left].
+          right with Monotemporary. left;constructor.
+          eright;[right;left;constructor|left].
+        * apply std_rel_rtc_Permanent in Hrtc;auto. subst.
+          apply revoke_lookup_Revoked in Hx as Hxtemp.
+          apply revoke_lookup_Perm in Hy as Hytemp.
+          simplify_eq. eright;[left;constructor|left].
+        * destruct h;revoke_i Wstd_sta Wstd_sta' i;try left;
+            try (right with Temporary;[left;constructor|eright;[right;right;constructor|left]]).
+          right with Temporary;[left;constructor|]. right with Revoked;[right;right;constructor|].
+          right with Monotemporary;[left;constructor|]. eright;[|left]. right;right;constructor.
+          right with Temporary;[left;constructor|]. right with Revoked;[right;right;constructor|].
+          right with Monotemporary;[left;constructor|]. eright;[|left]. right;left;constructor.
+        * subst. destruct h;revoke_i Wstd_sta Wstd_sta' i;try left;
+            try (right with Monotemporary;[left;constructor|eright;[right;right;constructor|left]]).
+          1,2: (right with Monotemporary;[left;constructor|right with Temporary;[right;right;constructor|]]).
+          eright;[right;right;constructor|left].
+          eright;[right;right;constructor|left].
+          right with Monotemporary;[left;constructor|].
+          eright;[|left]. right;left;constructor.
+        * subst. destruct h;revoke_i Wstd_sta Wstd_sta' i;try left;
+            try (right with Monotemporary;[left;constructor|eright;[right;right;constructor|left]]).
+          1,2: (right with Monotemporary;[left;constructor|right with Temporary;[right;right;constructor|]]).
+          eright;[right;right;constructor|left]. eright;[right;right;constructor|left].
+          right with Monotemporary;[left;constructor|].
+          eright;[|left]. right;left;constructor.
+      + destruct j,k,h; inversion Hjk; try discriminate; auto;
+          revoke_i Wstd_sta Wstd_sta' i; try left.
+        eright;[left;constructor|left].
+        right with Temporary;[left;constructor|eright;[right;right;constructor|left]].
+        right with Monotemporary;[left;constructor|eright;[right;right;constructor|left]].
+        right with Monotemporary;[left;constructor|eright;[right;left;constructor|left]].
       + destruct j,k,h; inversion Hjk; try discriminate; auto;
           revoke_i Wstd_sta Wstd_sta' i; try left;
-            [right with Temporary;[left;constructor|eright;[right;constructor|left] ]..].
+            try (right with Temporary;[left;constructor|eright;[right;right;constructor|left]]);
+            try (right with Monotemporary;[left;constructor|eright;[right;right;constructor|left]]);
+            try (right with Monotemporary;[left;constructor|eright;[right;left;constructor|left]]).
   Qed.
 
   Lemma revoke_monotone W W' :
@@ -725,23 +1006,40 @@ Section heap.
     rewrite /revoke_list /=.
     destruct (std W !! i) eqn:Hsome; auto.
     destruct r eqn:Htemp; auto.
-    destruct W as [ Wstd_sta Wloc].
-    destruct Hpriv as [(Hdoms & Ha) Hloc]; auto.
-    split;simpl;auto.
-    rewrite /related_sts_std_priv.
-    simpl in *.
-    split.
-    - rewrite dom_insert_L. set_solver.
-    - intros j x y Hx Hy.
-      destruct (decide (i = j)).
-      { subst.
-        rewrite lookup_insert in Hy. inversion Hy.
-        rewrite Hsome in Hx;inversion Hx;subst.
-        right with Revoked;[|left].
-        right. constructor.
-      }
-      rewrite lookup_insert_ne in Hy;auto.
-      apply Ha with j;auto.
+    - destruct W as [ Wstd_sta Wloc].
+      destruct Hpriv as [(Hdoms & Ha) Hloc]; auto.
+      split;simpl;auto.
+      rewrite /related_sts_std_priv.
+      simpl in *.
+      split.
+      + rewrite dom_insert_L. set_solver.
+      + intros j x y Hx Hy.
+        destruct (decide (i = j)).
+        { subst.
+          rewrite lookup_insert in Hy. inversion Hy.
+          rewrite Hsome in Hx;inversion Hx;subst.
+          right with Revoked;[|left].
+          right. right. constructor.
+        }
+        rewrite lookup_insert_ne in Hy;auto.
+        apply Ha with j;auto.
+    - destruct W as [ Wstd_sta Wloc].
+      destruct Hpriv as [(Hdoms & Ha) Hloc]; auto.
+      split;simpl;auto.
+      rewrite /related_sts_std_priv.
+      simpl in *.
+      split.
+      + rewrite dom_insert_L. set_solver.
+      + intros j x y Hx Hy.
+        destruct (decide (i = j)).
+        { subst.
+          rewrite lookup_insert in Hy. inversion Hy.
+          rewrite Hsome in Hx;inversion Hx;subst.
+          right with Revoked;[|left].
+          right. right. constructor.
+        }
+        rewrite lookup_insert_ne in Hy;auto.
+        apply Ha with j;auto.
   Qed.
 
   Lemma revoke_list_related_sts_priv W l :
@@ -771,10 +1069,9 @@ Section heap.
     - rewrite /revoke_list /=.
       destruct (std W !! a) eqn:Hsome; auto.
       destruct r eqn:Htemp;auto.
-      rewrite dom_insert_L. rewrite IHl.
-      assert (a ∈ dom (gset Addr) M) as Hin.
-      { rewrite -Hdom. apply elem_of_gmap_dom. eauto. }
-      set_solver.
+      all: rewrite dom_insert_L;rewrite IHl.
+      all: assert (a ∈ dom (gset Addr) M) as Hin;[rewrite -Hdom;apply elem_of_gmap_dom;eauto|].
+      all: try set_solver.
   Qed.
 
   (* ---------------------------------------------------------------------------------------- *)
@@ -798,6 +1095,13 @@ Section heap.
       iPureIntro.
       eapply revoke_lookup_non_temp; eauto.
     }
+    iAssert (∀ a ρ, ⌜m' !! a = Some ρ⌝ → ⌜ρ ≠ Monotemporary⌝)%I as %Hmonotemp.
+    { iIntros (a ρ Hsome).
+      iDestruct (big_sepM2_lookup_1 _ _ _ a with "Hstates") as (γp) "[Hl Hstate]"; eauto.
+      iDestruct (sts_full_state_std with "Hfull Hstate") as %Hρ.
+      iPureIntro.
+      eapply revoke_lookup_non_temp; eauto.
+    }
     iFrame.
     iApply big_sepM_exists. iExists m'.
     iApply big_sepM2_sep. iFrame.
@@ -805,10 +1109,11 @@ Section heap.
     iApply (big_sepM2_mono with "Hr").
     iIntros (a ρ γp Hm' HM) "/= [Hstate Ha]".
     specialize (Htemp a ρ Hm').
-    destruct ρ;iFrame;[contradiction|].
+    specialize (Hmonotemp a ρ Hm').
+    destruct ρ;iFrame;[contradiction|contradiction|].
     iDestruct "Ha" as (γpred p φ) "(Hγp & % & Hpred & Ha)".
     iDestruct "Ha" as (v) "(Hne & Ha & #Hmono & #Hφ)".
-    iExists _,_,_. iFrame "∗ #". iSplit;auto. iExists _; iFrame "∗ #".
+    iExists _,_,_;iFrame "∗ #"; iSplit;auto; iExists _; iFrame "∗ #".
     iNext. iApply ("Hmono" with "[] Hφ").
     iPureIntro. apply revoke_related_sts_priv.
     Unshelve. apply _.
@@ -832,13 +1137,21 @@ Section heap.
       iDestruct (sts_full_state_std with "Hfull Hstate") as %Hρ.
       iPureIntro. eapply revoke_lookup_non_temp; eauto.
     }
+    iAssert (∀ a ρ, ⌜m' !! a = Some ρ⌝ → ⌜ρ ≠ Monotemporary⌝)%I as %Hmonotemp.
+    { iIntros (a ρ Hsome).
+      iDestruct (big_sepM2_sep with "Hr") as "[Hstates Hr]".
+      iDestruct (big_sepM2_lookup_1 _ _ _ a with "Hstates") as (γp) "[_ Hstate]"; eauto.
+      iDestruct (sts_full_state_std with "Hfull Hstate") as %Hρ.
+      iPureIntro. eapply revoke_lookup_non_temp; eauto.
+    }
     iFrame.
     iApply big_sepM_exists. iExists m'.
     iApply big_sepM2_sep. iFrame.
     iApply (big_sepM2_mono with "Hr").
     iIntros (a ρ γp Hsomeρ Hsomeγp) "[Hstate Ha] /=".
     specialize (Htemp a ρ Hsomeρ).
-    destruct ρ;[contradiction|iFrame|iFrame|iFrame].
+    specialize (Hmonotemp a ρ Hsomeρ).
+    destruct ρ;try contradiction;iFrame.
     iDestruct "Ha" as (γpred p φ) "(Hγp & % & Hpred & Ha)".
     iDestruct "Ha" as (v) "(Hne & Ha & #Hmono & #Hφ)".
     iFrame.
@@ -867,7 +1180,16 @@ Section heap.
            ⌜p ≠ O⌝
           ∗ a ↦ₐ[p] v
           ∗ (if pwl p
-             then future_pub_mono φ v
+             then future_pub_plus_mono φ v
+             else future_priv_mono φ v)
+          ∗ φ (W,v))%I.
+
+  Definition monotemp_resources (W : WORLD) φ (a : Addr) (p : Perm) : iProp Σ :=
+    (∃ (v : Word),
+           ⌜p ≠ O⌝
+          ∗ a ↦ₐ[p] v
+          ∗ (if pwl p
+             then future_pub_a_mono a φ v
              else future_priv_mono φ v)
           ∗ φ (W,v))%I.
 
@@ -888,7 +1210,7 @@ Section heap.
   Qed.
 
   Lemma region_rel_get (W : WORLD) (a : Addr) :
-    (std W) !! a = Some Temporary ->
+    (std W) !! a = Some Temporary ∨ (std W) !! a = Some Monotemporary ->
     region W ∗ sts_full_world W ==∗
      region W ∗ sts_full_world W ∗ ∃ p φ, ⌜forall Wv, Persistent (φ Wv)⌝ ∗ rel a p φ.
   Proof.
@@ -897,63 +1219,113 @@ Section heap.
     iDestruct "Hr" as (M Mρ) "(HM & #Hdom & #Hdom' & Hr)".
     iDestruct "Hdom" as %Hdom. iDestruct "Hdom'" as %Hdom'.
     assert (is_Some (M !! a)) as [γp Hγp].
-    { apply elem_of_gmap_dom. rewrite -Hdom. apply elem_of_gmap_dom. eauto. }
+    { apply elem_of_gmap_dom. rewrite -Hdom. apply elem_of_gmap_dom. destruct Hlookup; eauto. }
     rewrite RELS_eq /RELS_def.
     iMod (reg_get with "[$HM]") as "[HM Hrel]";[eauto|].
     (* rewrite /region_map_def. iDestruct (reg_in with "[$HM $Hrel]") as %HMeq. *)
     iDestruct (big_sepM_delete _ _ a with "Hr") as "[Hstate Hr]";[eauto|].
     iDestruct "Hstate" as (ρ Ha) "[Hρ Hstate]".
     iDestruct (sts_full_state_std with "Hsts Hρ") as %Hx''.
-    rewrite Hlookup in Hx''. inversion Hx''. subst.
-    iDestruct "Hstate" as (γpred p φ Heq Hpers) "(#Hsaved & Ha)".
-    iDestruct "Ha" as (v Hne) "(Ha & Hmono & #Hφ)".
-    destruct γp as [γpred' p']; inversion Heq; subst.
-    iDestruct (big_sepM_delete _ _ a with "[Hρ Ha Hmono Hφ $Hr]") as "Hr";[eauto| |].
-    { iExists Temporary. iFrame. iSplit;auto. iExists γpred, p, φ. iFrame "∗ #". repeat iSplit; auto.
-      iExists _. iFrame "∗ #". auto. }
-    iModIntro.
-    iSplitL "HM Hr".
-    { iExists M. iFrame. auto. }
-    iFrame. iExists p,φ. iSplit;auto. rewrite rel_eq /rel_def REL_eq /REL_def. iExists γpred.
-    iFrame "Hsaved Hrel".
+    destruct Hlookup as [Hlookup | Hlookup].
+    all: rewrite Hlookup in Hx'';inversion Hx'';subst.
+    all: iDestruct "Hstate" as (γpred p φ Heq Hpers) "(#Hsaved & Ha)".
+    all: iDestruct "Ha" as (v Hne) "(Ha & Hmono & #Hφ)".
+    all: destruct γp as [γpred' p']; inversion Heq; subst.
+    all: iDestruct (big_sepM_delete _ _ a with "[Hρ Ha Hmono Hφ $Hr]") as "Hr";[eauto| |].
+    1: { iExists Temporary. iFrame. iSplit;auto. iExists γpred, p, φ. iFrame "∗ #". repeat iSplit; auto.
+         iExists _. iFrame "∗ #". auto. }
+    2: { iExists Monotemporary. iFrame. iSplit;auto. iExists γpred, p, φ. iFrame "∗ #". repeat iSplit; auto.
+         iExists _. iFrame "∗ #". auto. }
+    all: iModIntro.
+    all: iSplitL "HM Hr".
+    1: { iExists M. iFrame. auto. }
+    2: { iExists M. iFrame. auto. }
+    all: iFrame; iExists p,φ; iSplit;auto; rewrite rel_eq /rel_def REL_eq /REL_def; iExists γpred.
+    all: iFrame "Hsaved Hrel".
   Qed.
 
-  Lemma monotone_revoke_list_sts_full_world_keep W (l : list Addr) (l' : list Addr) :
-    ⊢ ⌜NoDup l'⌝ → ⌜NoDup l⌝ → ⌜l' ⊆+ l⌝ →
+  Lemma submseteq_NoDup {A : Type} (l l' : list A) : l' ⊆+ l → NoDup l -> NoDup l'.
+  Proof.
+    intros Hsub Hdup.
+    apply submseteq_Permutation in Hsub as [k Heq].
+    revert Hdup; rewrite Heq =>Hdup.
+    by apply NoDup_app in Hdup as (? & _ & _).
+  Qed.
+
+  Lemma monotone_revoke_list_sts_full_world_keep W (l : list Addr) (l' k' : list Addr) :
+    ⊢ ⌜NoDup (l)⌝ → ⌜l' ⊆+ l⌝ → ⌜k' ⊆+ l⌝  →
     ([∗ list] a ∈ l', ⌜(std W) !! a = Some Temporary⌝ (* ∧ rel a p φ *))
+    ∗ ([∗ list] a ∈ k', ⌜(std W) !! a = Some Monotemporary⌝ (* ∧ rel a p φ *))
     ∗ sts_full_world W ∗ region W
     ==∗ (sts_full_world (revoke_list l W) ∗ region W
-                        ∗ [∗ list] a ∈ l', ∃ p φ, ⌜forall Wv, Persistent (φ Wv)⌝ ∗ ▷ temp_resources W φ a p ∗ rel a p φ).
+                        ∗ ([∗ list] a ∈ l', ∃ p φ, ⌜forall Wv, Persistent (φ Wv)⌝ ∗ ▷ temp_resources W φ a p ∗ rel a p φ)
+                        ∗ ([∗ list] a ∈ k', ∃ p φ, ⌜forall Wv, Persistent (φ Wv)⌝ ∗ ▷ monotemp_resources W φ a p ∗ rel a p φ)).
   Proof.
     (* destruct W as [ [Wstd_sta Wstd_rel] Wloc].  *)
     rewrite /std region_eq /region_def /=.
-    iInduction (l) as [|x l] "IH" forall (l');
-    iIntros (Hdup' Hdup Hsub) "(#Hrel & Hfull & Hr)".
-    - iFrame. apply submseteq_nil_r in Hsub as ->. repeat rewrite big_sepL_nil. done.
-    - destruct (decide (x ∈ l')).
-      + apply elem_of_list_split in e as [l1 [l2 Heq] ].
-        rewrite Heq in Hsub.
-        iRevert (Hsub Hdup Hdup'). rewrite Heq -Permutation_middle. iIntros (Hsub Hdup Hdup').
-        apply NoDup_cons in Hdup as [Hnin Hdup].
-        apply NoDup_cons in Hdup' as [Hnin' Hdup'].
-        assert (x ∈ l') as Ha.
-        { rewrite Heq. apply elem_of_app. right. apply elem_of_list_here. }
-        apply elem_of_Permutation in Ha as [l'' Hleq].
-        simpl. iDestruct "Hrel" as "[ Htemp Hrel]".
-        iDestruct "Htemp" as %Htemp.
+    iInduction (l) as [|x l] "IH" forall (l' k');
+    iIntros (Hdup Hsub Hsubk) "(#Hrel & #Hrel' & Hfull & Hr)".
+    - apply submseteq_nil_r in Hsub as ->.
+      apply submseteq_nil_r in Hsubk as ->.
+      repeat rewrite big_sepL_nil. iFrame. done.
+    - destruct (decide (x ∈ l' ++ k')).
+      + iAssert (⌜∀ x0, (x0 ∈ l' → x0 ∉ k') ∧ (x0 ∈ k' → x0 ∉ l')⌝)%I as %Hdisj. 
+        { iIntros (x0). iSplit; iIntros (Hin Hcontr).
+          all: iDestruct (big_sepL_elem_of with "Hrel") as %Htemp;eauto.
+          all: iDestruct (big_sepL_elem_of with "Hrel'") as %Htemp';eauto.
+          all: congruence. }
+        iAssert (∃ l2' k2',
+                    ⌜NoDup l2' ∧ l2' ⊆+ l ∧ NoDup k2' ∧ k2' ⊆+ l ∧
+                    match W.1 !! x with
+                    | Some Temporary => l' ≡ₚx :: l2' ∧ k' ≡ₚk2'
+                    | Some Monotemporary => l' ≡ₚl2' ∧ k' ≡ₚx :: k2'
+                    | _ => False
+                    end⌝ ∧
+                    ([∗ list] a ∈ l2', ⌜W.1 !! a = Some Temporary⌝) ∗ ([∗ list] a ∈ k2', ⌜W.1 !! a = Some Monotemporary⌝))%I
+          as (l2' k2') "#[Hpure [Hrel2 Hrel2']]";[|iDestruct "Hpure" as %(Hdup2' & Hsub2 & Hdupk2' & Hdupk2 & Hmatch)].
+        { apply elem_of_app in e as [Hin | Hin].
+          - destruct Hdisj with x as [Hnin _]. specialize (Hnin Hin).
+            apply elem_of_Permutation in Hin as [l2' Heql2].
+            iExists l2',k'. iAssert ([∗ list] a ∈ (x :: l2'), ⌜W.1 !! a = Some Temporary⌝)%I as "#Hrel2";[rewrite Heql2;iFrame "Hrel"|].
+            simpl. iDestruct "Hrel2" as "[% $]". rewrite H0. iFrame "Hrel'". iPureIntro. apply NoDup_cons in Hdup as [Hninx Hdup].
+            apply submseteq_cons_r in Hsubk as [Hsubk | [k2' [Hk2' Hsubk2']]].
+            2: { exfalso. apply Hnin. rewrite Hk2'. apply elem_of_cons. by left. }
+            assert (l2' ⊆+ l).
+            { apply submseteq_cons_r in Hsub as [Hsub | [l'' [Hl'' Heql'']]].
+              + trans l';auto. rewrite Heql2. apply submseteq_cons;auto.
+              + trans l'';auto. apply Permutation_cons_inv in Heql2 as [l1 [l2 [Heq Hl']]].
+                subst. apply Permutation_sym,Permutation_cons_app_inv in Hl''. rewrite Hl' Hl''. done. }
+            repeat split;auto;eapply submseteq_NoDup;eauto.
+          - destruct Hdisj with x as [_ Hnin]. specialize (Hnin Hin).
+            apply elem_of_Permutation in Hin as [l2' Heql2].
+            iExists l',l2'. iAssert ([∗ list] a ∈ (x :: l2'), ⌜W.1 !! a = Some Monotemporary⌝)%I as "#Hrel2";[rewrite Heql2;iFrame "Hrel'"|].
+            simpl. iDestruct "Hrel2" as "[% $]". rewrite H0. iFrame "Hrel". iPureIntro. apply NoDup_cons in Hdup as [Hninx Hdup].
+            apply submseteq_cons_r in Hsub as [Hsub | [k2' [Hk2' Hsubk2']]].
+            2: { exfalso. apply Hnin. rewrite Hk2'. apply elem_of_cons. by left. }
+            assert (l2' ⊆+ l).
+            { apply submseteq_cons_r in Hsubk as [Hsubk | [l'' [Hl'' Heql'']]].
+              + trans k';auto. rewrite Heql2. apply submseteq_cons;auto.
+              + trans l'';auto. apply Permutation_cons_inv in Heql2 as [l1 [l2 [Heq Hl']]].
+                subst. apply Permutation_sym,Permutation_cons_app_inv in Hl''. rewrite Hl' Hl''. done. }
+            repeat split;auto;eapply submseteq_NoDup;eauto.
+        }
+        apply NoDup_cons in Hdup as [Hnin Hdup]. 
+        simpl.
+        iAssert (⌜W.1 !! x = Some Temporary ∨ W.1 !! x = Some Monotemporary⌝)%I as %Htemp.
+        { apply elem_of_app in e as [Hin | Hin].
+          - iDestruct (big_sepL_elem_of with "Hrel") as "Htemp";eauto. iLeft. auto.
+          - iDestruct (big_sepL_elem_of with "Hrel'") as "Htemp";eauto. iRight. auto. }
         iMod (region_rel_get with "[$Hfull Hr]") as "(Hfull & Hr & #Hx)";[apply Htemp|..].
         { rewrite region_eq /region_def. iFrame. }
         rewrite region_eq /region_def.
-        iMod ("IH" with "[] [] [] [$Hrel $Hfull $Hr]") as "(Hfull & Hr & Hl)"; auto.
-        { iPureIntro. apply submseteq_cons_l in Hsub as [k' [Hperm Hsub] ].
-          apply Permutation.Permutation_cons_inv in Hperm. etrans;eauto. rewrite Hperm. done. }
+        iMod ("IH" $! l2' k2' with "[] [] [] [$Hrel2 $Hrel2' $Hfull $Hr]") as "(Hfull & Hr & Hl & Hk)"; auto.
         rewrite /revoke_list /= /std /=.
-        rewrite Htemp.
         rewrite rel_eq /rel_def REL_eq RELS_eq /REL_def /RELS_def.
         iDestruct "Hr" as (M Mρ) "(HM & % & #Hdom & Hpreds)".
         iDestruct "Hdom" as %Hdom.
         iDestruct "Hx" as (p' φ' Hpers) "Hx".
         iDestruct "Hx" as (γpred) "#(Hγpred & Hφ)".
+
         (* assert that γrel = γrel' *)
         iDestruct (reg_in γrel (M) with "[$HM $Hγpred]") as %HMeq.
         rewrite /region_map_def.
@@ -963,11 +1335,13 @@ Section heap.
         iDestruct (sts_full_state_std with "Hfull Hstate") as %Hlookup.
         simpl in Hlookup.
         simpl in Hlookup. subst. rewrite revoke_list_not_elem_of_lookup in Hlookup; auto.
-        rewrite Htemp in Hlookup. inversion Hlookup. subst ρ.
         iMod (sts_update_std _ _ _ (Revoked) with "Hfull Hstate") as "[Hfull Hstate]".
-        iDestruct (region_map_delete_nonstatic with "Hpreds") as "Hpreds";[intros m; by rewrite Ha|].
+        iDestruct (region_map_delete_nonstatic with "Hpreds") as "Hpreds".
+        { intros m. destruct Htemp as [Htemp | Htemp]; rewrite Htemp in Hlookup;inversion Hlookup.
+          all: subst ρ; rewrite Ha;auto. }
         iDestruct (region_map_insert_nonstatic Revoked with "Hpreds") as "Hpreds";auto.
-        iFrame "∗ #". iClear "IH".
+        iClear "IH".
+        iSplitL "Hfull";[destruct Htemp as [-> | ->]; by iFrame|].
         iDestruct (big_sepM_insert _ _ x (γpred, p') with "[$Hpreds Hstate]") as "Hpreds"; [apply lookup_delete|..].
         iExists Revoked. iFrame. iSplitR. iPureIntro; apply lookup_insert.
         iExists _,_,_. iFrame "#". iSplit;auto.
@@ -978,46 +1352,60 @@ Section heap.
            assert (x ∈ dom (gset Addr) M) as Hin.
            { rewrite -Hdom. apply elem_of_gmap_dom. eauto. }
            revert Hin Hdom. clear; intros Hin Hdom. rewrite Hdom. set_solver.
-        ++ iExists p', φ'. iSplitR;auto. iSplitL.
-           +++ iDestruct "Ha" as (γpred0 p0 φ0 Heq0 Hpers0) "(#Hsaved & Ha)".
-               iDestruct "Ha" as (v Hne0) "(Hx & Hmono & #Hφ0)"; simplify_eq.
-               iExists v. destruct W as [ Wstd_sta Wloc].
-               iDestruct (saved_pred_agree _ _ _ (Wstd_sta, Wloc, v) with "Hφ Hsaved") as "#Hφeq". iFrame.
-               iSplitR; auto.
-               iDestruct (internal_eq_iff with "Hφeq") as "Hφeq'".
-               iSplitL "Hmono";[|by iNext; iApply "Hφeq'"].
-               destruct (pwl p0).
-               { iDestruct "Hmono" as "#Hmono".
-                 iApply later_intuitionistically_2. iModIntro.
-                 repeat (iApply later_forall_2; iIntros (W W')).
-                 iDestruct (saved_pred_agree _ _ _ (W', v) with "Hφ Hsaved") as "#HφWeq'".
-                 iDestruct (internal_eq_iff with "HφWeq'") as "HφWeq''".
-                 iDestruct (saved_pred_agree _ _ _ (W, v) with "Hφ Hsaved") as "#HφWeq".
-                 iDestruct (internal_eq_iff with "HφWeq") as "HφWeq'''".
-                 iModIntro. iIntros (Hrelated) "HφW". iApply "HφWeq''". iApply "Hmono"; eauto.
-                 iApply "HφWeq'''"; auto. }
-               { iDestruct "Hmono" as "#Hmono".
-                 iApply later_intuitionistically_2. iModIntro.
-                 repeat (iApply later_forall_2; iIntros (W W')).
-                 iDestruct (saved_pred_agree _ _ _ (W', v) with "Hφ Hsaved") as "#HφWeq'".
-                 iDestruct (internal_eq_iff with "HφWeq'") as "HφWeq''".
-                 iDestruct (saved_pred_agree _ _ _ (W, v) with "Hφ Hsaved") as "#HφWeq".
-                 iDestruct (internal_eq_iff with "HφWeq") as "HφWeq'''".
-                 iModIntro. iIntros (Hrelated) "HφW". iApply "HφWeq''". iApply "Hmono"; eauto.
-                 iApply "HφWeq'''"; auto. }
-           +++ iExists γpred. iFrame "#".
-      + apply NoDup_cons in Hdup as [Hnin Hdup].
-        apply submseteq_cons_r in Hsub as [Hsub | [l'' [Hcontr _] ] ].
-        2: { exfalso. apply n. rewrite Hcontr. apply elem_of_list_here. }
-        iMod ("IH" with "[] [] [] [$Hrel $Hfull $Hr]") as "(Hfull & Hr & Hl)"; auto.
+        ++
+          iAssert (∃ (p : Perm) (φ : WORLD * Word → iPropI Σ),
+                      ⌜∀ Wv : WORLD * Word, Persistent (φ Wv)⌝
+                      ∗ match W.1 !! x with
+                        | Some Temporary => ▷ temp_resources W φ x p
+                        | Some Monotemporary => ▷ monotemp_resources W φ x p
+                        | _ => False
+                        end
+                      ∗ (∃ γpred0 : gnameO, own γrel (◯ {[x := to_agree (γpred0, p)]}) ∗ saved_pred_own γpred0 φ))%I with "[Ha]" as "Ha".
+          { iExists p', φ'. iSplitR;auto. iSplitL.
+            - iDestruct "Ha" as (γpred0 p0 φ0 Heq0 Hpers0) "(#Hsaved & Ha)".
+              destruct Htemp as [Htemp | Htemp]; rewrite Htemp.
+              all: rewrite Htemp in Hlookup;inversion Hlookup.
+              all: iDestruct "Ha" as (v Hne0) "(Hx & Hmono & #Hφ0)"; simplify_eq.
+              all: iExists v;destruct W as [ Wstd_sta Wloc].
+              all: iDestruct (saved_pred_agree _ _ _ (Wstd_sta, Wloc, v) with "Hφ Hsaved") as "#Hφeq";iFrame.
+              all: iSplitR; auto.
+              all: iDestruct (internal_eq_iff with "Hφeq") as "Hφeq'".
+              all: iSplitL "Hmono";[|by iNext; iApply "Hφeq'"].
+              all: destruct (pwl p0).
+              all: iDestruct "Hmono" as "#Hmono".
+              all: iApply later_intuitionistically_2; iModIntro.
+              all: repeat (iApply later_forall_2; iIntros (W W')).
+              all: iDestruct (saved_pred_agree _ _ _ (W', v) with "Hφ Hsaved") as "#HφWeq'".
+              all: iDestruct (internal_eq_iff with "HφWeq'") as "HφWeq''".
+              all: iDestruct (saved_pred_agree _ _ _ (W, v) with "Hφ Hsaved") as "#HφWeq".
+              all: iDestruct (internal_eq_iff with "HφWeq") as "HφWeq'''".
+              all: iModIntro; iIntros (Hrelated) "HφW";iApply "HφWeq''"; iApply "Hmono"; eauto.
+              all: iApply "HφWeq'''"; auto.
+            - iExists γpred. iFrame "#". }
+          destruct Htemp as [Htemp | Htemp];rewrite Htemp in Hmatch.
+          all: destruct Hmatch as [-> ->];iFrame.
+          all: rewrite Htemp;iFrame.
+      + (* assert (Hdup_copy:=Hdup). *)
+        (* rewrite Heqlk in Hdup. *)
+        apply NoDup_cons in Hdup as [Hnin Hdup].
+        apply not_elem_of_app in n as [Hn1 Hn2].
+        iAssert (⌜l' ⊆+ l ∧ k' ⊆+ l ∧ NoDup l⌝)%I
+          as "#Hpure";[|iDestruct "Hpure" as %(Hsub2 & Hsubk2 & Hdup2)].
+        { iPureIntro. repeat split;auto.
+          - apply submseteq_cons_r in Hsub as [Hsubl | [k'' [Hperm Hk'']]];auto.
+            revert Hn1; rewrite Hperm =>Hn1. apply not_elem_of_cons in Hn1 as [Hcontr Hn1];contradiction.
+          - apply submseteq_cons_r in Hsubk as [Hsubl | [k'' [Hperm Hk'']]];auto.
+            revert Hn2; rewrite Hperm =>Hn2. apply not_elem_of_cons in Hn2 as [Hcontr Hn2];contradiction.
+        }
+        iMod ("IH" $! l' k' with "[] [] [] [$Hrel $Hrel' $Hfull $Hr]") as "(Hfull & Hr & $ & $)"; auto.
         iDestruct "Hr" as (M Mρ) "(HM & #Hdom & #Hdom' & Hr)".
         iDestruct "Hdom" as %Hdom. iDestruct "Hdom'" as %Hdom'. iClear "IH".
         rewrite /revoke_list /std /=. destruct W as [ Wstd_sta Wloc].
         destruct (Wstd_sta !! x) eqn:Hsome.
         2: { iFrame. iModIntro. rewrite Hsome. iFrame. iExists M. iFrame. auto. }
         rewrite Hsome.
-        destruct (decide (r = Temporary)).
-        2: { destruct r; try contradiction; iFrame; iModIntro; iExists M; iFrame; auto. }
+        destruct (decide (r = Temporary ∨ r = Monotemporary)).
+        2: { apply Decidable.not_or in n as [Hne Hne']. destruct r; try contradiction; iFrame; iModIntro; iExists M; iFrame; auto. }
         assert (is_Some (M !! x)) as [γp Hsomea].
         { apply elem_of_gmap_dom. rewrite -Hdom. apply elem_of_gmap_dom. eauto. }
         iDestruct (big_sepM_delete _ _ x with "Hr") as "[Hx Hr]"; eauto.
@@ -1026,118 +1414,133 @@ Section heap.
         iMod (sts_update_std _ _ _ (Revoked) with "Hfull Hstate") as "[Hfull Hstate]". iFrame.
         simpl in *. rewrite revoke_list_not_elem_of_lookup in Hlookup;auto.
         rewrite Hlookup in Hsome. inversion Hsome. subst.
-        iDestruct (region_map_delete_nonstatic with "Hr") as "Hpreds";[intros m; rewrite Ha; auto|].
+        iDestruct (region_map_delete_nonstatic with "Hr") as "Hpreds";[intros m; destruct o as [-> | ->]; rewrite Ha; auto|].
         iDestruct (region_map_insert_nonstatic Revoked with "Hpreds") as "Hpreds";auto.
         iDestruct (big_sepM_delete _ _ x with "[Hstate $Hpreds Hρ]") as "Hr"; eauto.
         iExists Revoked; iFrame. iSplitR. iPureIntro. apply lookup_insert.
         iDestruct "Hρ" as (? ? ? ? ?) "[? _]". iExists _,_,_. repeat iSplit;eauto.
-        iModIntro. iFrame. iExists M, _. iFrame.
-        iSplit; auto.
-        iPureIntro. rewrite dom_insert_L.
-        assert (x ∈ dom (gset Addr) M) as Hin.
-        { rewrite -Hdom'. apply elem_of_gmap_dom. eauto. }
-        revert Hin Hdom'. clear; intros Hin Hdom. rewrite Hdom. set_solver.
+        iModIntro. destruct o as [-> | ->]; iFrame;iExists M, _;iFrame.
+        all: iSplit; auto.
+        all:iPureIntro; rewrite dom_insert_L.
+        all: assert (x ∈ dom (gset Addr) M) as Hin.
+        1,3: rewrite -Hdom'; apply elem_of_gmap_dom; eauto.
+        all: revert Hin Hdom'. all: clear; intros Hin Hdom. all: rewrite Hdom. all: set_solver.
   Qed.
 
-  Lemma monotone_revoke_list_sts_full_world_keep_alt W (l : list Addr) (l' : list Addr) p φ :
-    ⊢ ⌜NoDup l'⌝ → ⌜NoDup l⌝ → ⌜l' ⊆+ l⌝ →
-    ([∗ list] a ∈ l', ⌜(std W) !! a = Some Temporary⌝ ∗ rel a p φ)
+  Lemma monotone_revoke_list_sts_full_world_keep_alt W (l : list Addr) (l' k' : list Addr) p φ :
+    ⊢ ⌜NoDup l⌝ → ⌜l' ⊆+ l⌝ → ⌜k' ⊆+ l⌝ →
+      ([∗ list] a ∈ l', ⌜(std W) !! a = Some Temporary⌝ ∗ rel a p φ)
+    ∗ ([∗ list] a ∈ k', ⌜(std W) !! a = Some Monotemporary⌝ ∗ rel a p φ)
     ∗ sts_full_world W ∗ region W
     ==∗ (sts_full_world (revoke_list l W) ∗ region W
-                        ∗ [∗ list] a ∈ l', ▷ temp_resources W φ a p ∗ rel a p φ).
+                        ∗ ([∗ list] a ∈ l', ▷ temp_resources W φ a p ∗ rel a p φ)
+                        ∗ ([∗ list] a ∈ k', ▷ monotemp_resources W φ a p ∗ rel a p φ)).
   Proof.
     (* destruct W as [ [Wstd_sta Wstd_rel] Wloc].  *)
-    iIntros (Hdupl Hdupl' Hsub) "(Htemp & Hsts & Hr)".
+    iIntros (Hdupl Hsub Hsubk) "(Htemp & Hmonotemp & Hsts & Hr)".
     iDestruct (big_sepL_sep with "Htemp") as "[Htemp Hrel]".
-    iMod (monotone_revoke_list_sts_full_world_keep with "[] [] [] [$Hsts $Hr $Htemp]") as "(Hsts & Hr & Htemp)";auto.
-    iFrame. iApply big_sepL_bupd.
-    iDestruct (big_sepL_sep with "[$Hrel $Htemp]") as "Htemp".
-    iApply (big_sepL_mono with "Htemp").
-    iIntros (k y Hsome) "(#Hr & Htemp)".
-    iDestruct "Htemp" as (p' φ' Hpers) "[Htemp #Hrel]".
-    iModIntro. rewrite /temp_resources.
-    iDestruct (rel_agree _ p p' with "[$Hrel $Hr]") as "(% & #Hφeq')".
-    subst.
-    iDestruct "Htemp" as (v) "(Hne & Ha & Hmono & Hφ)".
-    iFrame "Hr".
-    iExists v. iFrame "#". iFrame. iSplitL "Hmono".
-    - destruct (pwl p').
-      + iIntros (W' W'' Hrelated). iDestruct "Hmono" as "#Hmono".
-        iDestruct (rel_agree _ _ _ φ φ' with "[$Hrel $Hr]") as "(% & #Hφeq'')".
-        iSpecialize ("Hφeq'" $! (W',v)) .
-        iSpecialize ("Hφeq''" $! (W'',v)) .
-        iNext. iModIntro.
-        iRewrite "Hφeq''". iRewrite "Hφeq'".
-        iIntros "Hφ". iApply "Hmono"; eauto.
-      + iIntros (W' W'' Hrelated). iDestruct "Hmono" as "#Hmono".
-        iDestruct (rel_agree _ _ _ φ φ' with "[$Hrel $Hr]") as "(% & #Hφeq'')".
-        iSpecialize ("Hφeq'" $! (W',v)) .
-        iSpecialize ("Hφeq''" $! (W'',v)) .
-        iNext. iModIntro.
-        iRewrite "Hφeq''". iRewrite "Hφeq'".
-        iIntros "Hφ". iApply "Hmono"; eauto.
-    - iNext. iSpecialize ("Hφeq'" $! (W,v)). iRewrite "Hφeq'". iFrame.
+    iDestruct (big_sepL_sep with "Hmonotemp") as "[Hmonotemp Hmonorel]".
+    iMod (monotone_revoke_list_sts_full_world_keep with "[] [] [] [$Hsts $Hr $Htemp $Hmonotemp]") as "(Hsts & Hr & Htemp & Hmonotemp)";auto.
+    iFrame. iSplitL "Htemp Hrel".
+    all: iApply big_sepL_bupd.
+    1: iDestruct (big_sepL_sep with "[$Hrel $Htemp]") as "Htemp".
+    2: iDestruct (big_sepL_sep with "[$Hmonorel $Hmonotemp]") as "Htemp".
+    all: iApply (big_sepL_mono with "Htemp").
+    all: iIntros (k0 y Hsome) "(#Hr & Htemp)".
+    all: iDestruct "Htemp" as (p' φ' Hpers) "[Htemp #Hrel]".
+    all: iModIntro;rewrite /temp_resources /monotemp_resources.
+    all: iDestruct (rel_agree _ p p' with "[$Hrel $Hr]") as "(% & #Hφeq')".
+    all: subst.
+    all: iDestruct "Htemp" as (v) "(Hne & Ha & Hmono & Hφ)".
+    all: iFrame "Hr".
+    all: iExists v; iFrame "#"; iFrame. all: iSplitL "Hmono". 
+    1,3: destruct (pwl p').
+    5,6: iNext; iSpecialize ("Hφeq'" $! (W,v)); iRewrite "Hφeq'"; iFrame.
+    all: iIntros (W' W'' Hrelated); iDestruct "Hmono" as "#Hmono".
+    all: iDestruct (rel_agree _ _ _ φ φ' with "[$Hrel $Hr]") as "(% & #Hφeq'')".
+    all: iSpecialize ("Hφeq'" $! (W',v)) .
+    all: iSpecialize ("Hφeq''" $! (W'',v)) .
+    all: iNext; iModIntro.
+    all: iRewrite "Hφeq''"; iRewrite "Hφeq'".
+    all: iIntros "Hφ"; iApply "Hmono"; eauto.
   Qed.
 
-  Lemma monotone_revoke_sts_full_world_keep W (l : list Addr) :
-    ⌜NoDup l⌝ -∗
-    ([∗ list] a ∈ l, ⌜(std W) !! a = Some Temporary⌝)
-    ∗ sts_full_world W ∗ region W
+  Lemma monotone_revoke_sts_full_world_keep W (l k : list Addr) :
+    ⌜NoDup (l ++ k)⌝ -∗
+     ([∗ list] a ∈ l, ⌜(std W) !! a = Some Temporary⌝) ∗
+     ([∗ list] a ∈ k, ⌜(std W) !! a = Some Monotemporary⌝)
+     ∗ sts_full_world W ∗ region W
     ==∗ (sts_full_world (revoke W) ∗ region W ∗
-                        ([∗ list] a ∈ l, ∃ p φ, ⌜forall Wv, Persistent (φ Wv)⌝ ∗ ▷ temp_resources W φ a p ∗ rel a p φ)).
+                          ([∗ list] a ∈ l, ∃ p φ, ⌜forall Wv, Persistent (φ Wv)⌝ ∗ ▷ temp_resources W φ a p ∗ rel a p φ)
+                        ∗ ([∗ list] a ∈ k, ∃ p φ, ⌜forall Wv, Persistent (φ Wv)⌝ ∗ ▷ monotemp_resources W φ a p ∗ rel a p φ)).
   Proof.
-    iIntros (Hdup) "(Hl & Hfull & Hr)".
+    iIntros (Hdup) "(Hl & Hk & Hfull & Hr)".
     rewrite revoke_list_dom.
-    iAssert (⌜l ⊆+ (map_to_list W.1).*1⌝)%I as %Hsub.
-    { iClear "Hfull Hr". iInduction l as [| x l] "IH".
-      - iPureIntro. apply submseteq_nil_l.
-      - iDestruct "Hl" as "[ Hin Hl]".
-        iDestruct "Hin" as %Hin. apply NoDup_cons in Hdup as [Hnin Hdup].
-        iDestruct ("IH" with "[] Hl") as %Hsub; auto.
-        iPureIntro.
-        assert (x ∈ (map_to_list W.1).*1) as Helem.
-        { apply map_to_list_fst. exists Temporary. by apply elem_of_map_to_list. }
-        apply elem_of_Permutation in Helem as [l' Hl']. rewrite Hl'.
-        apply submseteq_skip. revert Hsub. rewrite Hl'; intros Hsub.
-        apply submseteq_cons_r in Hsub as [Hsub | [l'' [Heq _] ] ]; auto.
-        assert (countable.encode x ∈ countable.encode <$> l) as Hcontr.
-        { rewrite Heq. apply elem_of_list_here. }
-        apply elem_of_list_fmap_2 in Hcontr as [y [Hxy Hy] ].
-        apply encode_inj in Hxy. subst. contradiction.
+    iAssert (⌜l ⊆+ (map_to_list W.1).*1 ∧ k ⊆+ (map_to_list W.1).*1⌝)%I as %[Hsub Hsubk].
+    { iClear "Hfull Hr". iSplit.
+      1: iClear "Hk"; iInduction l as [| x l] "IH".
+      3: iClear "Hl"; iInduction k as [| x k] "IH".
+      1,3: iPureIntro;apply submseteq_nil_l.
+      1: iDestruct "Hl" as "[ Hin Hl]".
+      2: iDestruct "Hk" as "[ Hin Hl]".
+      all: iDestruct "Hin" as %Hin; simpl in *. 
+      2: revert Hdup; rewrite -Permutation_middle =>Hdup.
+      all: apply NoDup_cons in Hdup as [Hnin Hdup].
+      all: iDestruct ("IH" with "[] Hl") as %Hsub; auto.
+      all: iPureIntro.
+      all: assert (x ∈ (map_to_list W.1).*1) as Helem.
+      1,3: apply map_to_list_fst; eexists; by apply elem_of_map_to_list. 
+      all: apply elem_of_Permutation in Helem as [l' Hl']; rewrite Hl'.
+      all: apply submseteq_skip;revert Hsub; rewrite Hl'; intros Hsub.
+      all: apply submseteq_cons_r in Hsub as [Hsub | [l'' [Heq _] ] ]; auto.
+      1: assert (countable.encode x ∈ countable.encode <$> l) as Hcontr.
+      3: assert (countable.encode x ∈ countable.encode <$> k) as Hcontr.
+      1,3: rewrite Heq; apply elem_of_list_here.
+      all: apply elem_of_list_fmap_2 in Hcontr as [y [Hxy Hy] ].
+      all: apply encode_inj in Hxy; subst; apply not_elem_of_app in Hnin as [? ?];contradiction.
     }
-    iMod (monotone_revoke_list_sts_full_world_keep _ (map_to_list W.1).*1 l
-            with "[] [] [] [$Hl $Hfull $Hr]") as "(Hfull & Hr & Hi)"; auto.
+    iMod (monotone_revoke_list_sts_full_world_keep _ (map_to_list W.1).*1
+            with "[] [] [] [$Hl $Hfull $Hr $Hk]") as "(Hfull & Hr & Hi)"; auto.
     { iPureIntro. apply (NoDup_fst_map_to_list (M:=gmap Addr) (A:=region_type)). }
     iFrame. done.
   Qed.
 
-  Lemma monotone_revoke_sts_full_world_keep_alt W (l : list Addr) p φ :
-    ⌜NoDup l⌝ -∗
-    ([∗ list] a ∈ l, ⌜(std W) !! a = Some Temporary⌝ ∗ rel a p φ)
-    ∗ sts_full_world W ∗ region W
+  Lemma monotone_revoke_sts_full_world_keep_alt W (l k : list Addr) p φ :
+    ⌜NoDup (l ++ k)⌝ -∗
+     ([∗ list] a ∈ l, ⌜(std W) !! a = Some Temporary⌝ ∗ rel a p φ)
+     ∗ ([∗ list] a ∈ k, ⌜(std W) !! a = Some Monotemporary⌝ ∗ rel a p φ)
+     ∗ sts_full_world W ∗ region W
     ==∗ (sts_full_world (revoke W) ∗ region W ∗
-                        ([∗ list] a ∈ l, ▷ temp_resources W φ a p ∗ rel a p φ)).
+                        ([∗ list] a ∈ l, ▷ temp_resources W φ a p ∗ rel a p φ)
+                        ∗ ([∗ list] a ∈ k, ▷ monotemp_resources W φ a p ∗ rel a p φ)).
   Proof.
-    iIntros (Hdup) "(Hl & Hfull & Hr)".
+    iIntros (Hdup) "(Hl & Hk & Hfull & Hr)".
     rewrite revoke_list_dom.
-    iAssert (⌜l ⊆+ (map_to_list W.1).*1⌝)%I as %Hsub.
-    { iClear "Hfull Hr". iInduction l as [| x l] "IH".
-      - iPureIntro. apply submseteq_nil_l.
-      - iDestruct "Hl" as "[ [Hin Hrel] Hl]".
-        iDestruct "Hin" as %Hin. apply NoDup_cons in Hdup as [Hnin Hdup].
-        iDestruct ("IH" with "[] Hl") as %Hsub; auto.
-        iPureIntro.
-        assert (x ∈ (map_to_list W.1).*1) as Helem.
-        { apply map_to_list_fst. exists Temporary. by apply elem_of_map_to_list. }
-        apply elem_of_Permutation in Helem as [l' Hl']. rewrite Hl'.
-        apply submseteq_skip. revert Hsub. rewrite Hl'; intros Hsub.
-        apply submseteq_cons_r in Hsub as [Hsub | [l'' [Heq _] ] ]; auto.
-        assert (x ∈ l) as Hcontr.
-        { rewrite Heq. apply elem_of_list_here. }
-        subst. contradiction.
+    iAssert (⌜l ⊆+ (map_to_list W.1).*1 ∧ k ⊆+ (map_to_list W.1).*1⌝)%I as %[Hsub Hsubk].
+    { iClear "Hfull Hr". iSplit.
+      1: iClear "Hk"; iInduction l as [| x l] "IH".
+      3: iClear "Hl"; iInduction k as [| x k] "IH".
+      1,3: iPureIntro;apply submseteq_nil_l.
+      1: iDestruct "Hl" as "[ [Hin Hrel] Hl]".
+      2: iDestruct "Hk" as "[ [Hin Hrel] Hl]".
+      all: iDestruct "Hin" as %Hin; simpl in *. 
+      2: revert Hdup; rewrite -Permutation_middle =>Hdup.
+      all: apply NoDup_cons in Hdup as [Hnin Hdup].
+      all: iDestruct ("IH" with "[] Hl") as %Hsub; auto.
+      all: iPureIntro.
+      all: assert (x ∈ (map_to_list W.1).*1) as Helem.
+      1,3: apply map_to_list_fst; eexists; by apply elem_of_map_to_list. 
+      all: apply elem_of_Permutation in Helem as [l' Hl']; rewrite Hl'.
+      all: apply submseteq_skip;revert Hsub; rewrite Hl'; intros Hsub.
+      all: apply submseteq_cons_r in Hsub as [Hsub | [l'' [Heq _] ] ]; auto.
+      1: assert (countable.encode x ∈ countable.encode <$> l) as Hcontr.
+      3: assert (countable.encode x ∈ countable.encode <$> k) as Hcontr.
+      1,3: rewrite Heq; apply elem_of_list_here.
+      all: apply elem_of_list_fmap_2 in Hcontr as [y [Hxy Hy] ].
+      all: apply encode_inj in Hxy; subst; apply not_elem_of_app in Hnin as [? ?];contradiction.
     }
     iMod (monotone_revoke_list_sts_full_world_keep_alt _ (map_to_list W.1).*1 l
-            with "[] [] [] [$Hl $Hfull $Hr]") as "(Hfull & Hr & Hi)"; auto.
+            with "[] [] [] [$Hl $Hk $Hfull $Hr]") as "(Hfull & Hr & Hi)"; auto.
     { iPureIntro. apply (NoDup_fst_map_to_list (M:=gmap Addr) (A:=region_type)). }
     iFrame. done.
   Qed.
@@ -1161,25 +1564,27 @@ Section heap.
       { iPureIntro. intros a Ha. apply Hin. apply elem_of_cons. by right. }
       rewrite /revoke_list /= /std /=.
       destruct (Wstd_sta !! x) eqn:Hsome;[|iExists _; by iFrame].
-      destruct r;[|iExists _; by iFrame..].
-      destruct Hin with x as [γp Hsomea];[apply elem_of_list_here|].
-      iDestruct (big_sepM_delete _ _ x with "Hr") as "[Hρ Hr]"; eauto.
-      iDestruct "Hρ" as (ρ' Hρ') "(Hstate & Ha)".
-      iDestruct (sts_full_state_std with "Hfull Hstate") as %Hlookup.
-      simpl in Hlookup. subst. rewrite revoke_list_not_elem_of_lookup in Hlookup; auto.
-      rewrite Hsome in Hlookup. inversion Hlookup as [Heq]. subst ρ'.
-      iMod (sts_update_std _ _ _ (Revoked) with "Hfull Hstate") as "[Hfull Hstate]".
-      iFrame.
-      iDestruct (region_map_delete_nonstatic with "Hr") as "Hr";[intros m;by rewrite Hρ'|].
-      iDestruct (region_map_insert_nonstatic Revoked with "Hr") as "Hr";auto.
-      iExists _.
-      iDestruct "Ha" as (γpred p0 φ Heq Hpers) "[#Hsaved Ha]".
-      iDestruct (big_sepM_delete _ _ x with "[$Hr Hstate]") as "$"; eauto.
-      iExists Revoked. iFrame. iSplitR. iPureIntro. apply lookup_insert. iExists _,_,_. iFrame "#". iSplit;auto.
-      iPureIntro. rewrite -Hdom_new dom_insert_L.
-      assert (x ∈ dom (gset Addr) Mρ') as Hin'.
-      { apply elem_of_gmap_dom;eauto. }
-      set_solver.
+      destruct r;[| |iExists _; by iFrame..].
+      all: destruct Hin with x as [γp Hsomea];[apply elem_of_list_here|].
+      all: iDestruct (big_sepM_delete _ _ x with "Hr") as "[Hρ Hr]"; eauto.
+      all: iDestruct "Hρ" as (ρ' Hρ') "(Hstate & Ha)".
+      all: iDestruct (sts_full_state_std with "Hfull Hstate") as %Hlookup.
+      all: simpl in Hlookup; subst; rewrite revoke_list_not_elem_of_lookup in Hlookup; auto.
+      all: rewrite Hsome in Hlookup; inversion Hlookup as [Heq]; subst ρ'.
+      all: iMod (sts_update_std _ _ _ (Revoked) with "Hfull Hstate") as "[Hfull Hstate]".
+      all: iFrame.
+      all: iDestruct (region_map_delete_nonstatic with "Hr") as "Hr";[intros m;by rewrite Hρ'|].
+      all: iDestruct (region_map_insert_nonstatic Revoked with "Hr") as "Hr";auto.
+      all: iExists _.
+      all: iDestruct "Ha" as (γpred p0 φ Heq Hpers) "[#Hsaved Ha]".
+      all: iDestruct (big_sepM_delete _ _ x with "[$Hr Hstate]") as "$"; eauto.
+      1,3: iExists Revoked; iFrame; iSplitR.
+      all: try (iPureIntro; apply lookup_insert).
+      1,2: iExists _,_,_; iFrame "#"; iSplit;auto.
+      all: iPureIntro; rewrite -Hdom_new dom_insert_L.
+      all: assert (x ∈ dom (gset Addr) Mρ') as Hin'.
+      1,3: apply elem_of_gmap_dom;eauto. 
+      all: set_solver.
   Qed.
 
   (* The following statement discards all the resources of temporary regions *)
@@ -1206,12 +1611,12 @@ Section heap.
   Qed.
 
   Lemma submseteq_dom (l : list Addr) (Wstd_sta : gmap Addr region_type) :
-    Forall (λ i : Addr, Wstd_sta !! i = Some Temporary) l
+    Forall (λ i : Addr, Wstd_sta !! i = Some Temporary ∨ Wstd_sta !! i = Some Monotemporary) l
     → NoDup l → l ⊆+ (map_to_list Wstd_sta).*1.
   Proof.
     generalize l.
     induction Wstd_sta using map_ind.
-    + intros l' Htemps Hdup. destruct l'; auto. inversion Htemps. subst. discriminate.
+    + intros l' Htemps Hdup. destruct l'; auto. inversion Htemps. destruct H2; subst; discriminate.
     + intros l' Htemps Hdup. rewrite map_to_list_insert; auto.
       cbn.
       (* destruct on i being an element of l'! *)
@@ -1229,7 +1634,8 @@ Section heap.
              intros j Hin.
              assert (j ≠ i) as Hne.
              { intros Hcontr; subst. apply elem_of_app in Hin as [Hcontr | Hcontr]; congruence. }
-             rewrite -(Htemps j);[rewrite lookup_insert_ne;auto|].
+             destruct Htemps with j as [Htemp | Htemp]. 
+             2,3: rewrite -(Htemp);rewrite lookup_insert_ne;auto.
              subst. apply elem_of_app. apply elem_of_app in Hin as [Hin | Hin]; [left;auto|right].
              apply elem_of_cons;by right.
          +++ apply NoDup_app; repeat (split;auto).
@@ -1260,99 +1666,123 @@ Section heap.
   Qed.
 
   (* revoke and keep temp resources in list l, with unknown p and φ *)
-  Lemma monotone_revoke_keep W l :
-    NoDup l ->
+  Lemma monotone_revoke_keep W l k :
+    NoDup (l ++ k) ->
     ([∗ list] a ∈ l, ⌜(std W) !! a = Some Temporary⌝)
+      ∗ ([∗ list] a ∈ k, ⌜(std W) !! a = Some Monotemporary⌝)
       ∗ sts_full_world W ∗ region W ==∗ sts_full_world (revoke W) ∗ region (revoke W)
-      ∗ [∗ list] a ∈ l, (∃ p φ, ⌜forall Wv, Persistent (φ Wv)⌝ ∗ ▷ temp_resources W φ a p ∗ rel a p φ)
-                     ∗ ⌜(std (revoke W)) !! a = Some Revoked⌝.
+      ∗ ([∗ list] a ∈ l, (∃ p φ, ⌜forall Wv, Persistent (φ Wv)⌝ ∗ ▷ temp_resources W φ a p ∗ rel a p φ)
+                           ∗ ⌜(std (revoke W)) !! a = Some Revoked⌝)
+      ∗ ([∗ list] a ∈ k, (∃ p φ, ⌜forall Wv, Persistent (φ Wv)⌝ ∗ ▷ monotemp_resources W φ a p ∗ rel a p φ)
+                           ∗ ⌜(std (revoke W)) !! a = Some Revoked⌝).
   Proof.
-    iIntros (Hdup) "(Hl & HW & Hr)".
+    iIntros (Hdup) "(Hl & Hk & HW & Hr)".
     iAssert (⌜Forall (λ a, std W !! a = Some Temporary) l⌝)%I as %Htemps.
     { iDestruct (big_sepL_forall with "Hl") as %Htemps.
       iPureIntro. apply Forall_lookup. done. }
-    iMod (monotone_revoke_sts_full_world_keep with "[] [$HW $Hr $Hl]") as "(HW & Hr & Hl)"; eauto.
+    iAssert (⌜Forall (λ a, std W !! a = Some Monotemporary) k⌝)%I as %Hmonotemps.
+    { iDestruct (big_sepL_forall with "Hk") as %Hmonotemps.
+      iPureIntro. apply Forall_lookup. done. }
+    iMod (monotone_revoke_sts_full_world_keep with "[] [$HW $Hr $Hl $Hk]") as "(HW & Hr & Hl & Hk)"; eauto.
     rewrite region_eq /region_def.
     iDestruct "Hr" as (M Mρ) "(HM & % & % & Hpreds)".
     iDestruct (monotone_revoke_region_def with "[] [$HW] [$Hpreds]") as "[Hpreds HW]"; auto.
     iModIntro. iFrame. iSplitL "HW HM".
     - iExists _,_. iFrame. iPureIntro. split;auto. rewrite /revoke -revoke_dom_eq /=. auto.
-    - iApply big_sepL_sep. iFrame. iApply big_sepL_forall. iPureIntro.
-      revert Htemps. rewrite (Forall_lookup _ l). intros Hl i a Ha; auto.
-      specialize (Hl i a Ha). rewrite /revoke. apply revoke_lookup_Temp. done.
+    - iSplitL "Hl".
+      all: iApply big_sepL_sep; iFrame; iApply big_sepL_forall; iPureIntro.
+      1: revert Htemps. 2: revert Hmonotemps. 1: rewrite (Forall_lookup _ l). 2: rewrite (Forall_lookup _ k).
+      all: intros Hl i a Ha; auto.
+      all: specialize (Hl i a Ha). all: rewrite /revoke. by apply revoke_lookup_Temp. by apply revoke_lookup_Monotemp.
+      Unshelve. apply _.
   Qed.
 
   (* revoke and keep temp resources in list l, with know p and φ *)
-  Lemma monotone_revoke_keep_alt W l p φ :
-    NoDup l ->
+  Lemma monotone_revoke_keep_alt W l k p φ :
+    NoDup (l ++ k) ->
     ([∗ list] a ∈ l, ⌜(std W) !! a = Some Temporary⌝ ∗ rel a p φ)
+      ∗ ([∗ list] a ∈ k, ⌜(std W) !! a = Some Monotemporary⌝ ∗ rel a p φ)
       ∗ sts_full_world W ∗ region W ==∗ sts_full_world (revoke W) ∗ region (revoke W)
-      ∗ [∗ list] a ∈ l, (▷ temp_resources W φ a p ∗ rel a p φ)
-                     ∗ ⌜(std (revoke W)) !! a = Some Revoked⌝.
+      ∗ ([∗ list] a ∈ l, (▷ temp_resources W φ a p ∗ rel a p φ)
+                           ∗ ⌜(std (revoke W)) !! a = Some Revoked⌝)
+      ∗ ([∗ list] a ∈ k, (▷ monotemp_resources W φ a p ∗ rel a p φ)
+                           ∗ ⌜(std (revoke W)) !! a = Some Revoked⌝).
   Proof.
-    iIntros (Hdup) "(Hl & HW & Hr)".
+    iIntros (Hdup) "(Hl & Hk & HW & Hr)".
     iAssert (⌜Forall (λ a, std W !! a = Some Temporary) l⌝)%I as %Htemps.
     { iDestruct (big_sepL_sep with "Hl") as "[Htemps Hrel]".
       iDestruct (big_sepL_forall with "Htemps") as %Htemps.
       iPureIntro. apply Forall_lookup. done. }
-    iMod (monotone_revoke_sts_full_world_keep_alt with "[] [$HW $Hr $Hl]") as "(HW & Hr & Hl)"; eauto.
+    iAssert (⌜Forall (λ a, std W !! a = Some Monotemporary) k⌝)%I as %Hmonotemps.
+    { iDestruct (big_sepL_sep with "Hk") as "[Htemps Hrel]".
+      iDestruct (big_sepL_forall with "Htemps") as %Hmonotemps.
+      iPureIntro. apply Forall_lookup. done. }
+    iMod (monotone_revoke_sts_full_world_keep_alt with "[] [$HW $Hr $Hl $Hk]") as "(HW & Hr & Hl & Hk)"; eauto.
     rewrite region_eq /region_def.
     iDestruct "Hr" as (M Mρ) "(HM & % & % & Hpreds)".
     iDestruct (monotone_revoke_region_def with "[] [$HW] [$Hpreds]") as "[Hpreds HW]"; auto.
     iModIntro. iFrame. iSplitL "HW HM".
     - iExists _,_. iFrame. iPureIntro. split;auto. rewrite /revoke -revoke_dom_eq /=. auto.
-    - iApply big_sepL_sep. iFrame. iApply big_sepL_forall. iPureIntro.
-      revert Htemps. rewrite (Forall_lookup _ l). intros Hl i a Ha; auto.
-      specialize (Hl i a Ha). rewrite /revoke. apply revoke_lookup_Temp. done.
+    - iSplitL "Hl".
+      all: iApply big_sepL_sep. all: iFrame. all: iApply big_sepL_forall. all: iPureIntro.
+      1: revert Htemps. 2: revert Hmonotemps. 1: rewrite (Forall_lookup _ l). 2: rewrite (Forall_lookup _ k).
+      all: intros Hl i a Ha; auto.
+      all: specialize (Hl i a Ha). all: rewrite /revoke. by apply revoke_lookup_Temp. by apply revoke_lookup_Monotemp.
+      Unshelve. apply _. 
   Qed.
 
   (* For practical reasons, it will be convenient to have a version of revoking where you only know what some of the
-     temp regions are *)
-  Lemma monotone_revoke_keep_some W l1 l2 p φ :
-    NoDup (l1 ++ l2) ->
+     temp/monotemp regions are *)
+  Lemma monotone_revoke_keep_some W l1 l2 k1 k2 p φ :
+    NoDup (l1 ++ l2 ++ k1 ++ k2) ->
     ([∗ list] a ∈ l1, ⌜(std W) !! a = Some Temporary⌝) ∗
-    ([∗ list] a ∈ l2, ⌜(std W) !! a = Some Temporary⌝ ∗ rel a p φ)
-      ∗ sts_full_world W ∗ region W ==∗ sts_full_world (revoke W) ∗ region (revoke W)
-      ∗ ([∗ list] a ∈ l1, (∃ p φ, ⌜forall Wv, Persistent (φ Wv)⌝ ∗ ▷ temp_resources W φ a p ∗ rel a p φ)
-                           ∗ ⌜(std (revoke W)) !! a = Some Revoked⌝)
-      ∗ [∗ list] a ∈ l2, (▷ temp_resources W φ a p ∗ rel a p φ)
-                           ∗ ⌜(std (revoke W)) !! a = Some Revoked⌝.
+    ([∗ list] a ∈ l2, ⌜(std W) !! a = Some Temporary⌝ ∗ rel a p φ) ∗
+    ([∗ list] a ∈ k1, ⌜(std W) !! a = Some Monotemporary⌝) ∗
+    ([∗ list] a ∈ k2, ⌜(std W) !! a = Some Monotemporary⌝ ∗ rel a p φ)
+    ∗ sts_full_world W ∗ region W ==∗ sts_full_world (revoke W) ∗ region (revoke W)
+    ∗ ([∗ list] a ∈ l1, (∃ p φ, ⌜forall Wv, Persistent (φ Wv)⌝ ∗ ▷ temp_resources W φ a p ∗ rel a p φ)
+                          ∗ ⌜(std (revoke W)) !! a = Some Revoked⌝)
+    ∗ ([∗ list] a ∈ l2, (▷ temp_resources W φ a p ∗ rel a p φ)
+                          ∗ ⌜(std (revoke W)) !! a = Some Revoked⌝)
+    ∗ ([∗ list] a ∈ k1, (∃ p φ, ⌜forall Wv, Persistent (φ Wv)⌝ ∗ ▷ monotemp_resources W φ a p ∗ rel a p φ)
+                          ∗ ⌜(std (revoke W)) !! a = Some Revoked⌝)
+    ∗ ([∗ list] a ∈ k2, (▷ monotemp_resources W φ a p ∗ rel a p φ)
+                          ∗ ⌜(std (revoke W)) !! a = Some Revoked⌝).
   Proof.
-    iIntros (Hdup) "(Hl1 & Hl2 & HW & Hr)".
+    iIntros (Hdup) "(Hl1 & Hl2 & Hk1 & Hk2 & HW & Hr)".
     iDestruct (big_sepL_sep with "Hl2") as "[Hl2 #Hrels]".
+    iDestruct (big_sepL_sep with "Hk2") as "[Hk2 #Hrelsk]".
     iDestruct (big_sepL_app with "[$Hl1 $Hl2]") as "Hl".
-    iMod (monotone_revoke_keep with "[$HW $Hr $Hl]") as "(HW & Hr & Hl)";[auto|].
+    iDestruct (big_sepL_app with "[$Hk1 $Hk2]") as "Hk".
+    iMod (monotone_revoke_keep with "[$HW $Hr $Hl $Hk]") as "(HW & Hr & Hl & Hk)";[rewrite -app_assoc; auto|].
     iDestruct (big_sepL_app with "Hl") as "[Hl1 Hl2]".
     iDestruct (big_sepL_sep with "Hl2") as "[Hl2 Hrev]".
-    iFrame. iApply big_sepL_sep. iFrame.
-    iModIntro.
-    iDestruct (big_sepL_sep with "[Hrels $Hl2]") as "Hl2";[iFrame "Hrels"|].
-    iApply (big_sepL_mono with "Hl2").
-    iIntros (k y Hlookup) "[Htemp #Hrel]".
-    iDestruct "Htemp" as (p' φ' Hpers) "(Htemp & #Hrel')".
-    rewrite /temp_resources.
-    iDestruct (later_exist with "Htemp") as (v) "(Hne & Hy & Hmono & Hφ')".
-    iDestruct (rel_agree _ p p' with "[$Hrel $Hrel']") as (Heq) "#Hφeq". subst.
-    iFrame "Hrel". iApply later_exist_2. iExists (v). iFrame.
-    iSplitR "Hφ'".
-    - destruct (pwl p').
-      + iIntros (W' W'' Hrelated). iDestruct "Hmono" as "#Hmono".
-        iDestruct (rel_agree _ _ _ φ φ' with "[$Hrel $Hrel']") as "(% & #Hφeq')".
-        iSpecialize ("Hφeq'" $! (W',v)) .
-        iSpecialize ("Hφeq" $! (W'',v)) .
-        iNext. iModIntro.
-        iRewrite "Hφeq'". iRewrite "Hφeq".
-        iIntros "Hφ". iApply "Hmono"; eauto.
-      + iIntros (W' W'' Hrelated). iDestruct "Hmono" as "#Hmono".
-        iDestruct (rel_agree _ _ _ φ φ' with "[$Hrel $Hrel']") as "(% & #Hφeq')".
-        iSpecialize ("Hφeq'" $! (W',v)) .
-        iSpecialize ("Hφeq" $! (W'',v)) .
-        iNext. iModIntro.
-        iRewrite "Hφeq'". iRewrite "Hφeq".
-        iIntros "Hφ". iApply "Hmono"; eauto.
-    - iNext.
-      iSpecialize ("Hφeq" $! (W,v)).
-      iRewrite "Hφeq". iFrame.
+    iDestruct (big_sepL_app with "Hk") as "[Hk1 Hk2]".
+    iDestruct (big_sepL_sep with "Hk2") as "[Hk2 Hrevk]".
+    iFrame. iSplitL "Hl2 Hrev".
+    all: iApply big_sepL_sep; iFrame.
+    all: iModIntro.
+    1: iDestruct (big_sepL_sep with "[Hrels $Hl2]") as "Hl2";[iFrame "Hrels"|].
+    2: iDestruct (big_sepL_sep with "[Hrelsk $Hk2]") as "Hk2";[iFrame "Hrelsk"|].
+    1: iApply (big_sepL_mono with "Hl2").
+    2: iApply (big_sepL_mono with "Hk2").
+    all: iIntros (k y Hlookup) "[Htemp #Hrel]".
+    all: iDestruct "Htemp" as (p' φ' Hpers) "(Htemp & #Hrel')".
+    all: rewrite /temp_resources /monotemp_resources.
+    all: iDestruct (later_exist with "Htemp") as (v) "(Hne & Hy & Hmono & Hφ')".
+    all: iDestruct (rel_agree _ p p' with "[$Hrel $Hrel']") as (Heq) "#Hφeq"; subst.
+    all: iFrame "Hrel"; iApply later_exist_2; iExists (v); iFrame.
+    all: iSplitR "Hφ'".
+    1,3: destruct (pwl p').
+    5,6: iNext; iSpecialize ("Hφeq" $! (W,v)); iRewrite "Hφeq"; iFrame.
+    all: iIntros (W' W'' Hrelated); iDestruct "Hmono" as "#Hmono".
+    all: iDestruct (rel_agree _ _ _ φ φ' with "[$Hrel $Hrel']") as "(% & #Hφeq')".
+    all: iSpecialize ("Hφeq'" $! (W',v)) .
+    all: iSpecialize ("Hφeq" $! (W'',v)) .
+    all: iNext; iModIntro.
+    all: iRewrite "Hφeq'"; iRewrite "Hφeq".
+    all: iIntros "Hφ"; iApply "Hmono"; eauto.
+    Unshelve. apply _.
   Qed.
 
   (* ---------------------------------------------------------------------------------------- *)
@@ -1365,49 +1795,88 @@ Section heap.
      and no other address is temp*)
 
   Lemma extract_temps W :
-    ∃ l, NoDup l ∧ (forall (a : Addr), (std W) !! a = Some Temporary <-> a ∈ l).
+    ∃ l k, NoDup (l ++ k)
+           ∧ (forall (a : Addr), (std W) !! a = Some Temporary <-> a ∈ l)
+           ∧ (forall (a : Addr), (std W) !! a = Some Monotemporary <-> a ∈ k).
   Proof.
     destruct W as [Wstd_sta Wloc ].
     rewrite /std /=.
     induction Wstd_sta using (map_ind (M:=gmap Addr) (A:=region_type)).
-    - exists []. split;[by apply NoDup_nil|]. intros a. split; intros Hcontr; inversion Hcontr.
-    - destruct IHWstd_sta as [l [Hdup Hiff] ].
+    - exists [],[]. split;[by apply NoDup_nil|]. split; intros a; split; intros Hcontr; inversion Hcontr.
+    - destruct IHWstd_sta as [l [k [Hdup [Hiff Hiffk] ] ] ].
       assert (i ∈ dom (gset Addr) (<[i:=x]> m)) as Hin.
       { apply elem_of_dom. rewrite lookup_insert; eauto. }
       assert (i ∉ l) as Hnin.
       { intros Hcontr. apply Hiff in Hcontr. simplify_map_eq. }
+      assert (i ∉ k) as Hnin'.
+      { intros Hcontr. apply Hiffk in Hcontr. simplify_map_eq. }
+      assert (Hdup_copy:=Hdup).
+      apply NoDup_app in Hdup_copy as [Hdupl [Hdisj Hdupk] ].
       destruct (decide (x = Temporary)); subst.
-      + exists (i :: l). split;[apply NoDup_cons;split;auto|].
-        intros a0. destruct (decide (i = a0)); subst.
-        { rewrite lookup_insert. split; auto. intros _. apply elem_of_cons. by left. }
-        rewrite lookup_insert_ne;[|intros Hcontr;congruence].
+      + exists (i :: l),k. simpl. split;[apply NoDup_cons;split;auto;apply not_elem_of_app;auto|].
+        split;intros a0; destruct (decide (i = a0)); subst;simplify_map_eq.
+        1,3: rewrite lookup_insert.
+        { split;auto. intros _. apply elem_of_cons; by left. }
+        { split;intros Hcontr;[inversion Hcontr|]. congruence. }
+        1,2: rewrite lookup_insert_ne;[|intros Hcontr;congruence].
         split; intros Htemp.
         { apply elem_of_cons; right. by apply Hiff. }
         { apply elem_of_cons in Htemp as [Hcontr | Hin'];[congruence|]. apply Hiff; auto. }
-      + exists l. split; auto. intros a0. split.
-        { destruct (decide (i = a0));subst.
-          - rewrite lookup_insert. intros Hcontr. congruence.
-          - rewrite lookup_insert_ne;[apply Hiff|]. auto.
-        }
-        intros Hin'. destruct (decide (i = a0));[congruence|].
-        rewrite lookup_insert_ne;[|intros Hcontr;congruence].
-        apply Hiff; auto.
+        split;intros Htemp; by apply Hiffk. 
+      + destruct (decide (x = Monotemporary)); subst.
+        * exists l,(i::k). simpl. rewrite -Permutation_middle. split;[apply NoDup_cons;split;auto;apply not_elem_of_app;auto|].
+          split;intros a0; destruct (decide (i = a0)); subst;simplify_map_eq.
+          1,3: rewrite lookup_insert.
+          { split;intros Hcontr;[inversion Hcontr|]. congruence. }
+          { split;auto. intros _. apply elem_of_cons; by left. }
+          1,2: rewrite lookup_insert_ne;[|intros Hcontr;congruence].
+          split; intros Htemp; by apply Hiff.
+          split; intros Htemp.
+          { apply elem_of_cons; right. by apply Hiffk. }
+          { apply elem_of_cons in Htemp as [Hcontr | Hin'];[congruence|]. apply Hiffk; auto. }
+        * exists l,k. split; auto. split;intros a0. all: split.
+          1,3: destruct (decide (i = a0));subst.
+          1,3: rewrite lookup_insert; intros Hcontr; congruence.
+          1: rewrite lookup_insert_ne;[apply Hiff|]; auto.
+          1: rewrite lookup_insert_ne;[apply Hiffk|]; auto.
+          all: intros Hin'; destruct (decide (i = a0));[congruence|].
+          all: rewrite lookup_insert_ne;[|intros Hcontr;congruence].
+          apply Hiff; auto. apply Hiffk;auto.
   Qed.
 
   (* We also want to be able to split the extracted temporary regions into known and unknown *)
-  Lemma extract_temps_split W l :
-    NoDup l ->
+  Lemma extract_temps_split W l k :
+    NoDup (l ++ k) ->
     Forall (λ (a : Addr), (std W) !! a = Some Temporary) l ->
-    ∃ l', NoDup (l' ++ l) ∧ (forall (a : Addr), (std W) !! a = Some Temporary <-> a ∈ (l' ++ l)).
+    Forall (λ (a : Addr), (std W) !! a = Some Monotemporary) k ->
+    ∃ l' k', NoDup (l' ++ l ++ k' ++ k)
+             ∧ (forall (a : Addr), (std W) !! a = Some Temporary <-> a ∈ (l' ++ l))
+             ∧ (forall (a : Addr), (std W) !! a = Some Monotemporary <-> a ∈ (k' ++ k)).
   Proof.
-    intros Hdup HForall.
-    pose proof (extract_temps W) as [l' [Hdup' Hl'] ].
-    revert HForall; rewrite Forall_forall =>HForall.
-    exists (list_difference l' l). split.
-    - apply NoDup_app. split;[|split].
-      + apply NoDup_list_difference. auto.
-      + intros a Ha. apply elem_of_list_difference in Ha as [_ Ha]; auto.
-      + auto.
+    intros Hdup HForall HForallk.
+    pose proof (extract_temps W) as [l' [k' [Hdup' [Hl' Hk'] ]] ].
+    revert HForall HForallk; rewrite !Forall_forall =>HForall HForallk.
+    exists (list_difference l' l),(list_difference k' k). split;[|split].
+    - rewrite app_assoc. apply NoDup_app. split;[|split].
+      + apply NoDup_app. split;[|split].
+        * apply NoDup_list_difference. apply NoDup_app in Hdup' as [? ?]; auto.
+        * intros a Ha. apply elem_of_list_difference in Ha as [_ Ha]; auto.
+        * apply NoDup_app in Hdup as [? ?]; auto.
+      + intros a Ha. apply elem_of_app in Ha as [Ha | Ha].
+        * intros Hcontr. apply elem_of_app in Hcontr as [Hcontr | Hcontr].
+          ** apply elem_of_list_difference in Ha as [Ha _]; auto.
+             apply elem_of_list_difference in Hcontr as [Hcontr _]; auto.
+             apply NoDup_app in Hdup' as [_ [Hdup' _] ]. apply Hdup' in Ha. done.
+          ** apply elem_of_list_difference in Ha as [Ha' Ha]; auto.
+             apply HForallk in Hcontr. apply Hl' in Ha'.  congruence.
+        * intros Hcontr. apply elem_of_app in Hcontr as [Hcontr | Hcontr].
+          ** apply elem_of_list_difference in Hcontr as [Hcontr _]; auto.
+             apply HForall in Ha. apply Hk' in Hcontr. congruence.
+          ** apply NoDup_app in Hdup as [_ [Hdup _] ]. apply Hdup in Ha. done.
+      + apply NoDup_app. split;[|split].
+        * apply NoDup_list_difference. apply NoDup_app in Hdup' as [? [? ?] ]; auto.
+        * intros a Ha. apply elem_of_list_difference in Ha as [_ Ha]; auto.
+        * apply NoDup_app in Hdup as [? [? ?] ]; auto.
     - intros a. split.
       + intros Htemp.
         destruct (decide (a ∈ list_difference l' l));[by apply elem_of_app;left|].
@@ -1420,6 +1889,18 @@ Section heap.
         ++ apply elem_of_list_difference in Hin as [Hinl Hninl'].
            by apply Hl'.
         ++ by apply HForall.
+    - intros a. split.
+      + intros Htemp.
+        destruct (decide (a ∈ list_difference k' k));[by apply elem_of_app;left|].
+        apply elem_of_app;right. apply Hk' in Htemp.
+        assert (not (a ∈ k' ∧ a ∉ k)) as Hnot.
+        { intros Hcontr. apply elem_of_list_difference in Hcontr. contradiction. }
+        destruct (decide (a ∈ k)); auto.
+        assert (a ∈ k' ∧ a ∉ k) as Hcontr; auto. apply Hnot in Hcontr. done.
+      + intros Hin. apply elem_of_app in Hin as [Hin | Hin].
+        ++ apply elem_of_list_difference in Hin as [Hinl Hninl'].
+           by apply Hk'.
+        ++ by apply HForallk.
   Qed.
 
 
@@ -1427,22 +1908,35 @@ Section heap.
   (* ------------------ WE CAN UPDATE A REVOKED WORLD BACK TO TEMPORARY  -------------------- *)
   (* ---------------------------------------------------------------------------------------- *)
 
-  (* closing will take every revoked element of l and reinstate it as temporary *)
-  Fixpoint close_list_std_sta (l : list Addr) (fs : STS_STD) : STS_STD :=
+  (* closing will take every revoked element of l and reinstate it as Temporary,
+     and every revoked element of k and reinstate it as Monotemporary. l and k
+     are assumed to be disjoint *)
+  Fixpoint close_list_std_sta_temp (l : list Addr) (fs : STS_STD) : STS_STD :=
     match l with
     | [] => fs
     | i :: l' => match fs !! i with
                | Some j => match j with
-                          | Revoked => <[i := Temporary]> (close_list_std_sta l' fs)
-                          | _ => (close_list_std_sta l' fs)
+                          | Revoked => <[i := Temporary]> (close_list_std_sta_temp l' fs)
+                          | _ => (close_list_std_sta_temp l' fs)
                           end
-               | None => (close_list_std_sta l' fs)
-               end
+               | None => (close_list_std_sta_temp l' fs)
+                 end
     end.
-  Definition close_list l W : WORLD := (close_list_std_sta l (std W), loc W).
+  Fixpoint close_list_std_sta_monotemp (l : list Addr) (fs : STS_STD) : STS_STD :=
+    match l with
+    | [] => fs
+    | i :: l' => match fs !! i with
+               | Some j => match j with
+                          | Revoked => <[i := Monotemporary]> (close_list_std_sta_monotemp l' fs)
+                          | _ => (close_list_std_sta_monotemp l' fs)
+                          end
+               | None => (close_list_std_sta_monotemp l' fs)
+                 end
+    end.
+  Definition close_list l k W : WORLD := (close_list_std_sta_temp l (close_list_std_sta_monotemp k (std W)), loc W).
 
-  Lemma close_list_std_sta_is_Some Wstd_sta l i :
-    is_Some (Wstd_sta !! i) <-> is_Some (close_list_std_sta l Wstd_sta !! i).
+  Lemma close_list_std_sta_temp_is_Some Wstd_sta l i :
+    is_Some (Wstd_sta !! i) <-> is_Some (close_list_std_sta_temp l Wstd_sta !! i).
   Proof.
     split.
     - induction l.
@@ -1465,34 +1959,84 @@ Section heap.
         * rewrite lookup_insert_ne in Hx;eauto.
   Qed.
 
-  Lemma close_list_std_sta_None Wstd_sta l i :
-    Wstd_sta !! i = None <-> close_list_std_sta l Wstd_sta !! i = None.
+  Lemma close_list_std_sta_monotemp_is_Some Wstd_sta l i :
+    is_Some (Wstd_sta !! i) <-> is_Some (close_list_std_sta_monotemp l Wstd_sta !! i).
+  Proof.
+    split.
+    - induction l.
+      + done.
+      + intros [x Hx].
+      simpl.
+      destruct (Wstd_sta !! a);[|apply IHl;eauto].
+      destruct r;try (apply IHl;eauto).
+      destruct (decide (a = i)).
+        * subst. rewrite lookup_insert. eauto.
+        * rewrite lookup_insert_ne;eauto.
+    - induction l.
+      + done.
+      + intros [x Hx].
+        simpl in Hx.
+        destruct (Wstd_sta !! a) eqn:Hsome;eauto.
+        destruct r;try by (apply IHl;eauto).
+        destruct (decide (a = i)).
+        * subst. eauto.
+        * rewrite lookup_insert_ne in Hx;eauto.
+  Qed.
+
+  Lemma close_list_std_sta_temp_None Wstd_sta l i :
+    Wstd_sta !! i = None <-> close_list_std_sta_temp l Wstd_sta !! i = None.
   Proof.
     split.
     - intros Hnone. apply eq_None_not_Some.
-      intros Hcontr. apply close_list_std_sta_is_Some in Hcontr.
+      intros Hcontr. apply close_list_std_sta_temp_is_Some in Hcontr.
       apply eq_None_not_Some in Hcontr; auto.
     - intros Hnone. apply eq_None_not_Some.
-      intros Hcontr. revert Hcontr. rewrite close_list_std_sta_is_Some =>Hcontr.
+      intros Hcontr. revert Hcontr. rewrite close_list_std_sta_temp_is_Some =>Hcontr.
       apply eq_None_not_Some in Hcontr; eauto.
   Qed.
 
-  Lemma close_list_dom_eq Wstd_sta l :
-    dom (gset Addr) Wstd_sta = dom (gset Addr) (close_list_std_sta l Wstd_sta).
+  Lemma close_list_std_sta_monotemp_None Wstd_sta l i :
+    Wstd_sta !! i = None <-> close_list_std_sta_monotemp l Wstd_sta !! i = None.
+  Proof.
+    split.
+    - intros Hnone. apply eq_None_not_Some.
+      intros Hcontr. apply close_list_std_sta_monotemp_is_Some in Hcontr.
+      apply eq_None_not_Some in Hcontr; auto.
+    - intros Hnone. apply eq_None_not_Some.
+      intros Hcontr. revert Hcontr. rewrite close_list_std_sta_monotemp_is_Some =>Hcontr.
+      apply eq_None_not_Some in Hcontr; eauto.
+  Qed.
+
+  Lemma close_list_dom_eq_temp Wstd_sta l :
+    dom (gset Addr) Wstd_sta = dom (gset Addr) (close_list_std_sta_temp l Wstd_sta).
   Proof.
     apply gset_leibniz. split.
     - intros Hin.
       apply elem_of_gmap_dom. apply elem_of_gmap_dom in Hin.
-      rewrite -close_list_std_sta_is_Some.
+      rewrite -close_list_std_sta_temp_is_Some.
       eauto.
     - intros Hin.
       apply elem_of_gmap_dom. apply elem_of_gmap_dom in Hin.
-      rewrite close_list_std_sta_is_Some.
+      rewrite close_list_std_sta_temp_is_Some.
       eauto.
   Qed.
 
-  Lemma close_list_std_sta_same Wstd_sta l i :
-    i ∉ l → Wstd_sta !! i = close_list_std_sta l Wstd_sta !! i.
+  Lemma close_list_dom_eq_monotemp Wstd_sta l :
+    dom (gset Addr) Wstd_sta = dom (gset Addr) (close_list_std_sta_monotemp l Wstd_sta).
+  Proof.
+    apply gset_leibniz. split.
+    - intros Hin.
+      apply elem_of_gmap_dom. apply elem_of_gmap_dom in Hin.
+      rewrite -close_list_std_sta_monotemp_is_Some.
+      eauto.
+    - intros Hin.
+      apply elem_of_gmap_dom. apply elem_of_gmap_dom in Hin.
+      rewrite close_list_std_sta_monotemp_is_Some.
+      eauto.
+  Qed.
+
+  Lemma close_list_std_sta_same_temp Wstd_sta l i :
+    i ∉ l → Wstd_sta !! i = close_list_std_sta_temp l Wstd_sta !! i.
   Proof.
     intros Hnin. induction l.
     - done.
@@ -1502,9 +2046,20 @@ Section heap.
       rewrite lookup_insert_ne; auto.
   Qed.
 
-  Lemma close_list_std_sta_same_alt Wstd_sta l i :
+  Lemma close_list_std_sta_same_monotemp Wstd_sta l i :
+    i ∉ l → Wstd_sta !! i = close_list_std_sta_monotemp l Wstd_sta !! i.
+  Proof.
+    intros Hnin. induction l.
+    - done.
+    - simpl. apply not_elem_of_cons in Hnin as [Hne Hnin].
+      destruct (Wstd_sta !! a); auto.
+      destruct r; auto.
+      rewrite lookup_insert_ne; auto.
+  Qed.
+
+  Lemma close_list_std_sta_same_alt_temp Wstd_sta l i :
     Wstd_sta !! i ≠ Some Revoked ->
-    Wstd_sta !! i = close_list_std_sta l Wstd_sta !! i.
+    Wstd_sta !! i = close_list_std_sta_temp l Wstd_sta !! i.
   Proof.
     intros Hnin. induction l.
     - done.
@@ -1516,9 +2071,23 @@ Section heap.
       + rewrite lookup_insert_ne; auto.
   Qed.
 
-  Lemma close_list_std_sta_revoked Wstd_sta l i :
+  Lemma close_list_std_sta_same_alt_monotemp Wstd_sta l i :
+    Wstd_sta !! i ≠ Some Revoked ->
+    Wstd_sta !! i = close_list_std_sta_monotemp l Wstd_sta !! i.
+  Proof.
+    intros Hnin. induction l.
+    - done.
+    - simpl. (* apply not_elem_of_cons in Hnin as [Hne Hnin].  *)
+      destruct (Wstd_sta !! a) eqn:some; auto.
+      destruct r; auto.
+      destruct (decide (a = i)).
+      + subst. contradiction.
+      + rewrite lookup_insert_ne; auto.
+  Qed.
+
+  Lemma close_list_std_sta_temp_revoked Wstd_sta l i :
     i ∈ l -> Wstd_sta !! i = Some Revoked →
-    close_list_std_sta l Wstd_sta !! i = Some Temporary.
+    close_list_std_sta_temp l Wstd_sta !! i = Some Temporary.
   Proof.
     intros Hin Hrev. induction l.
     - inversion Hin.
@@ -1532,37 +2101,31 @@ Section heap.
         * rewrite lookup_insert_ne;auto.
   Qed.
 
-  Lemma std_rel_pub_not_temp_cases x y :
-    std_rel_pub x y ->
-    (x = Revoked ∧ y = Temporary) ∨
-    (∃ m, x = (Static m) ∧ y = Temporary).
+  Lemma close_list_std_sta_monotemp_revoked Wstd_sta l i :
+    i ∈ l -> Wstd_sta !! i = Some Revoked →
+    close_list_std_sta_monotemp l Wstd_sta !! i = Some Monotemporary.
   Proof.
-    intros Hpub.
-    inversion Hpub;subst;[left|right];auto. exists m. split;auto.
+    intros Hin Hrev. induction l.
+    - inversion Hin.
+    - apply elem_of_cons in Hin as [Heq | Hin].
+      + subst. simpl. rewrite Hrev.
+        rewrite lookup_insert. auto.
+      + simpl. destruct (Wstd_sta !! a); auto.
+        destruct r; auto.
+        destruct (decide (i = a)); subst.
+        * rewrite lookup_insert; auto.
+        * rewrite lookup_insert_ne;auto.
   Qed.
 
-  Lemma std_rel_pub_rtc_not_temp_cases x y :
-    rtc std_rel_pub x y ->
-    (x = Revoked ∧ y = Temporary) ∨
-    (∃ m, x = (Static m) ∧ y = Temporary) ∨
-    x = y.
-  Proof.
-    intros Hrtc.
-    destruct Hrtc as [|ρ y z Hrel].
-    - right. by (repeat right).
-    - apply std_rel_pub_not_temp_cases in Hrel as [ [Heq1 Heq2] | [m [Heq1 Heq2] ] ]; subst.
-      left. apply std_rel_pub_rtc_Temporary in Hrtc; auto.
-      right;left. apply std_rel_pub_rtc_Temporary in Hrtc; eauto.
-  Qed.
 
-  Lemma close_list_related_sts_pub_cons W a l :
-    related_sts_pub_world W (close_list l W) →
-    related_sts_pub_world W (close_list_std_sta (a :: l) (std W), loc W).
+  Lemma close_list_related_sts_pub_cons_temp W a l :
+    related_sts_pub_world W (close_list_std_sta_temp l (std W), loc W) →
+    related_sts_pub_world W (close_list_std_sta_temp (a :: l) (std W), loc W).
   Proof.
     rewrite /close_list /=. intros IHl.
     destruct (std W !! a) eqn:Hsome; auto.
     destruct r;auto.
-    apply related_sts_pub_trans_world with (close_list l W); auto.
+    apply related_sts_pub_trans_world with (close_list_std_sta_temp l (std W),loc W); auto.
     split;[|apply related_sts_pub_refl].
     split.
     + simpl. rewrite dom_insert /close_list /=.
@@ -1573,21 +2136,105 @@ Section heap.
       ++ rewrite lookup_insert in Hy. inversion Hy.
          subst.
          destruct (decide (a ∈ l)).
-         +++ apply close_list_std_sta_revoked with _ l _ in Hsome;auto.
+         +++ apply close_list_std_sta_temp_revoked with _ l _ in Hsome;auto.
              rewrite Hsome in Hx. inversion Hx. left.
-         +++ rewrite (close_list_std_sta_same _ l) in Hsome;auto.
+         +++ rewrite (close_list_std_sta_same_temp _ l) in Hsome;auto.
              rewrite Hsome in Hx. inversion Hx. right with Temporary;[|left].
              constructor.
       ++ rewrite lookup_insert_ne in Hy; auto.
          rewrite Hx in Hy. inversion Hy. left.
   Qed.
 
-  Lemma close_list_related_sts_pub W l :
-    related_sts_pub_world W (close_list l W).
+  Lemma close_list_related_sts_pub_cons_monotemp W a l :
+    related_sts_pub_world W (close_list_std_sta_monotemp l (std W), loc W) →
+    related_sts_pub_world W (close_list_std_sta_monotemp (a :: l) (std W), loc W).
+  Proof.
+    rewrite /close_list /=. intros IHl.
+    destruct (std W !! a) eqn:Hsome; auto.
+    destruct r;auto.
+    apply related_sts_pub_trans_world with (close_list_std_sta_monotemp l (std W),loc W); auto.
+    split;[|apply related_sts_pub_refl].
+    split.
+    + simpl. rewrite dom_insert /close_list /=.
+      apply union_subseteq_r.
+    + rewrite /close_list /=.
+      intros i x y Hx Hy.
+      destruct (decide (i = a)); subst.
+      ++ rewrite lookup_insert in Hy. inversion Hy.
+         subst.
+         destruct (decide (a ∈ l)).
+         +++ apply close_list_std_sta_monotemp_revoked with _ l _ in Hsome;auto.
+             rewrite Hsome in Hx. inversion Hx. left.
+         +++ rewrite (close_list_std_sta_same_monotemp _ l) in Hsome;auto.
+             rewrite Hsome in Hx. inversion Hx. right with Monotemporary;[|left].
+             constructor.
+      ++ rewrite lookup_insert_ne in Hy; auto.
+         rewrite Hx in Hy. inversion Hy. left.
+  Qed.
+
+  (*
+  Lemma close_list_related_sts_pub_cons_nested W a a0 l k :
+    related_sts_pub_world W (close_list l (a0 :: k) W) →
+    related_sts_pub_world W (close_list (a :: l) (a0 :: k) W).
+  Proof.
+    rewrite /close_list /=. intros IHl.
+    destruct (std W !! a) eqn:Hsome; auto.
+    destruct r;auto.
+    apply related_sts_pub_trans_world with (close_list_std_sta_monotemp l (std W),loc W); auto.
+    split;[|apply related_sts_pub_refl].
+    split.
+    + simpl. rewrite dom_insert /close_list /=.
+      apply union_subseteq_r.
+    + rewrite /close_list /=.
+      intros i x y Hx Hy.
+      destruct (decide (i = a)); subst.
+      ++ rewrite lookup_insert in Hy. inversion Hy.
+         subst.
+         destruct (decide (a ∈ l)).
+         +++ apply close_list_std_sta_monotemp_revoked with _ l _ in Hsome;auto.
+             rewrite Hsome in Hx. inversion Hx. left.
+         +++ rewrite (close_list_std_sta_same_monotemp _ l) in Hsome;auto.
+             rewrite Hsome in Hx. inversion Hx. right with Monotemporary;[|left].
+             constructor.
+      ++ rewrite lookup_insert_ne in Hy; auto.
+         rewrite Hx in Hy. inversion Hy. left.
+  Qed.
+
+
+  Lemma close_list_related_sts_pub_temp W l :
+    related_sts_pub_world W (close_list_std_sta_temp l W.1,loc W).
   Proof.
     induction l.
     - rewrite /close_list /=. destruct W. apply related_sts_pub_refl_world.
-    - apply close_list_related_sts_pub_cons; auto.
+    - apply close_list_related_sts_pub_cons_temp; auto. 
+  Qed.
+  Lemma close_list_related_sts_pub_monotemp W l :
+    related_sts_pub_world W (close_list_std_sta_monotemp l W.1,loc W).
+  Proof.
+    induction l.
+    - rewrite /close_list /=. destruct W. apply related_sts_pub_refl_world.
+    - apply close_list_related_sts_pub_cons_monotemp; auto. 
+  Qed.
+
+  Lemma close_list_related_sts_pub W l k :
+    related_sts_pub_world W (close_list l k W).
+  Proof.
+    induction l,k.
+    - rewrite /close_list /=. destruct W; apply related_sts_pub_refl_world.
+    - apply close_list_related_sts_pub_monotemp; auto.
+    - apply close_list_related_sts_pub_temp.
+    - 
+    - intros k'. eapply related_sts_pub_trans_world;eauto.
+      rewrite /close_list. 
+      apply close_list_related_sts_pub_cons_temp; eauto.
+      rewrite -/close_list. 
+      apply close_list_related_sts_pub_cons_temp; auto.
+    - 
+      apply close_list_related_sts_pub_cons_monotemp; eauto.
+      apply close_list_related_sts_pub_monotemp; eauto.
+      eapply related_sts_pub_trans_world;eauto. 
+      apply close_list_related_sts_pub_cons_temp; eauto.
+      apply close_list_related_sts_pub_temp; eauto.
   Qed.
 
   Lemma close_list_related_sts_pub_insert' Wstd_sta Wloc i l :
@@ -1620,49 +2267,6 @@ Section heap.
     apply related_sts_pub_trans_world with (close_list_std_sta l ((std (Wstd_sta, Wloc))), Wloc).
     - apply close_list_related_sts_pub.
     - apply close_list_related_sts_pub_insert'; auto.
-  Qed.
-
-  Lemma close_monotone W W' l :
-    related_sts_pub_world W W' → related_sts_pub_world (close_list l W) (close_list l W').
-  Proof.
-    intros Hrelated.
-    destruct W as [ Wstd_sta [Wloc_sta Wloc_rel] ].
-    destruct W' as [ Wstd_sta' [Wloc_sta' Wloc_rel'] ].
-    destruct Hrelated as [ [Hstd_sta_dom Hstd_related] Hloc_related ].
-    simpl in *.
-    rewrite /close_list /std /=.
-    split;[simpl|apply Hloc_related].
-    split;[repeat rewrite -close_list_dom_eq;auto|].
-    intros i x y Hx Hy.
-    destruct (decide (Wstd_sta !! i = Some Revoked)).
-    - destruct (decide (i ∈ l)).
-      + assert (is_Some (Wstd_sta' !! i)) as [y' Hy'];[rewrite close_list_std_sta_is_Some;eauto|].
-        specialize (Hstd_related i _ _ e Hy').
-        apply (close_list_std_sta_revoked _ l _) in e; auto. rewrite e in Hx.
-        inversion Hx; subst.
-        apply std_rel_pub_rtc_Revoked in Hstd_related as [Htemp | Hrev];auto.
-        ++ subst.
-           assert (close_list_std_sta l Wstd_sta' !! i = Some Temporary) as Hytemp.
-           { rewrite -(close_list_std_sta_same_alt _ l _); auto. rewrite Hy'. intros Hcontr. inversion Hcontr as [Heq]. }
-           rewrite Hy in Hytemp. inversion Hytemp. left.
-        ++ subst.
-           apply (close_list_std_sta_revoked _ l _) in Hy'; auto. rewrite Hy' in Hy.
-           inversion Hy. left.
-      + rewrite -close_list_std_sta_same in Hx; auto.
-        rewrite -close_list_std_sta_same in Hy; auto. apply Hstd_related with i;auto.
-    - rewrite -close_list_std_sta_same_alt in Hx; auto.
-      assert (is_Some (Wstd_sta' !! i)) as [y' Hy'];[rewrite close_list_std_sta_is_Some;eauto|].
-      specialize (Hstd_related _ _ _ Hx Hy').
-      apply std_rel_pub_rtc_not_temp_cases in Hstd_related as [ [Hcontr _]|Htemp].
-      + subst. congruence.
-      + subst.
-        assert (Wstd_sta' !! i ≠ Some Revoked) as Hneq.
-        { intros Hcontr. rewrite Hcontr in Hy'. inversion Hy'. subst.
-          destruct Htemp as [ [m [Heq1 Heq2] ] | Heq]. done. subst. done. }
-        rewrite -close_list_std_sta_same_alt in Hy; auto.
-        rewrite Hy in Hy'. inversion Hy'.
-        destruct Htemp as [ [m [Heq1 Heq2] ] | Heq]; subst; [..|left].
-        right with Temporary;[|left]. constructor.
   Qed.
 
   Lemma close_revoke_iff Wstd_sta (l : list Addr) :
@@ -1898,6 +2502,6 @@ Section heap.
     { apply close_list_dom_eq. }
     iDestruct (region_monotone _ _ Heq Hrelated' with "Hr") as "Hr". clear Hrelated'.
     iMod (close_list_consolidate _ _ l with "[] [] [$Hr $Hsts $Htemp]") as "[Hsts Hr]";[auto|eauto|iFrame;done].
-  Qed.
+  Qed.*)
 
 End heap.
